start playing around with recursive types

theories/rust_typing/type.v
@@ -35,7 +35,7 @@ Proof.
   rewrite /num_cred/num_laters_per_step /=. lia.
 Qed.
 
-(** Types are defined semantically by what it means for a value to have a particular type. 
+(** Types are defined semantically by what it means for a value to have a particular type.
     Types are indexed by their refinement type [rt].
 *)
 Record type `{!typeGS Σ} (rt : Type) := {
@@ -973,3 +973,162 @@ Section subtyping.
 
 
 End subtyping.
+
+
+
+(** Special metric for type-nonexpansive and Type-contractive functions. *)
+Section type_dist2.
+  Context `{!typeGS Σ}.
+  (* Metrics all assume one fixed refinement type *)
+  Context {rt : Type}.
+
+  (* Size and shr are n-equal, but own is only n-1-equal.
+     We need this to express what shr has to satisfy on a Type-NE-function:
+     It may only depend contractively on own. *)
+  (* TODO: Find a better name for this metric. *)
+  Inductive type_dist2 (n : nat) (ty1 ty2 : type rt) : Prop :=
+    Type_dist2 :
+      (*ty1.(ty_syn_type) = ty2.(ty_syn_type) →*)
+      (*ty1.(ty_lfts) = ty2.(ty_lfts) →*)
+      (*ty1.(ty_wf_E) = ty2.(ty_wf_E) →*)
+      (*(@inhabitant rt (ty1.(ty_rt_inhabited))) = (@inhabitant rt (ty2.(ty_rt_inhabited))) →*)
+      (*(∀ ot mt, ty_has_op_type ty1 ot mt ↔ ty_has_op_type ty2 ot mt) →*)
+      (∀ π r vs, dist_later n (ty1.(ty_own_val) π r vs) (ty2.(ty_own_val) π r vs)) →
+      (∀ κ π r l, ty1.(ty_shr) κ π r l ≡{n}≡ ty2.(ty_shr) κ π r l) →
+      (*(ty1.(ty_sidecond) ≡{n}≡ ty2.(ty_sidecond)) →*)
+      (*(∀ π r, ty1.(ty_ghost_drop) π r ≡{n}≡ ty2.(ty_ghost_drop) π r) →*)
+      type_dist2 n ty1 ty2.
+
+  Global Instance type_dist2_equivalence n : Equivalence (type_dist2 n).
+  Proof.
+    constructor.
+    - by constructor.
+    - intros ?? Heq; constructor; symmetry; eapply Heq.
+    - intros ??? Heq1 Heq2; constructor; etrans; (eapply Heq1 || eapply Heq2).
+  Qed.
+
+  Definition type_dist2_later (n : nat) ty1 ty2 : Prop :=
+    match n with O => True | S n => type_dist2 n ty1 ty2 end.
+  Global Arguments type_dist2_later !_ _ _ /.
+
+  Global Instance type_dist2_later_equivalence n :
+    Equivalence (type_dist2_later n).
+  Proof. destruct n as [|n]; first by split. apply type_dist2_equivalence. Qed.
+
+  (* The hierarchy of metrics:
+     dist n → type_dist2 n → dist_later n → type_dist2_later n. *)
+  Lemma type_dist_dist2 n ty1 ty2 :
+    dist n ty1 ty2 → type_dist2 n ty1 ty2.
+  Proof. intros EQ. split; intros; try apply dist_dist_later; apply EQ. Qed.
+  Lemma type_dist2_dist_later n ty1 ty2 :
+    type_dist2 n ty1 ty2 → dist_later n ty1 ty2.
+  Proof.
+    intros EQ. eapply dist_later_fin_iff. destruct n; first done.
+    split; intros; try apply EQ; try si_solver.
+    (*all: apply dist_S, EQ.*)
+  (*Qed.*)
+  Abort.
+  Lemma type_later_dist2_later n ty1 ty2 :
+    dist_later n ty1 ty2 → type_dist2_later n ty1 ty2.
+  Proof.
+    destruct n; first done. rewrite dist_later_fin_iff. exact: type_dist_dist2.
+  Qed.
+  Lemma type_dist2_dist n ty1 ty2 :
+    type_dist2 (S n) ty1 ty2 → dist n ty1 ty2.
+  Proof.
+    (*move=>/type_dist2_dist_later. rewrite dist_later_fin_iff. done.*)
+  (*Qed.*)
+  Abort.
+  Lemma type_dist2_S n ty1 ty2 :
+    type_dist2 (S n) ty1 ty2 → type_dist2 n ty1 ty2.
+  Proof.
+    (*intros. apply type_dist_dist2, type_dist2_dist. done. *)
+  (*Qed.*)
+  Abort.
+
+  (*
+  Lemma ty_size_type_dist n : Proper (type_dist2 n ==> eq) ty_size.
+  Proof. intros ?? EQ. apply EQ. Qed.
+  Lemma ty_own_type_dist n:
+    Proper (type_dist2 (S n) ==> eq ==> eq ==> dist n) ty_own.
+  Proof. intros ?? EQ ??-> ??->. apply EQ. si_solver. Qed.
+  Lemma ty_shr_type_dist n :
+    Proper (type_dist2 n ==> eq ==> eq ==> eq ==> dist n) ty_shr.
+  Proof. intros ?? EQ ??-> ??-> ??->. apply EQ. Qed.
+  *)
+End type_dist2.
+
+(** Type-nonexpansive and Type-contractive functions. *)
+(* Note that TypeContractive is neither weaker nor stronger than Contractive, because
+   (a) it allows the dependency of own on shr to be non-expansive, and
+   (b) it forces the dependency of shr on own to be doubly-contractive.
+   It would be possible to weaken this so that no double-contractivity is required.
+   However, then it is no longer possible to write TypeContractive as just a
+   Proper, which makes it significantly more annoying to use.
+   For similar reasons, TypeNonExpansive is incomparable to NonExpansive.
+*)
+Notation TypeNonExpansive T := (∀ n, Proper (type_dist2 n ==> type_dist2 n) T).
+Notation TypeContractive T := (∀ n, Proper (type_dist2_later n ==> type_dist2 n) T).
+
+Section type_contractive.
+  Context `{!typeGS Σ}.
+  Context {rt1 rt2 rt3 : Type}.
+
+  Lemma type_ne_dist_later (T : type rt1 → type rt2) :
+    TypeNonExpansive T → ∀ n, Proper (type_dist2_later n ==> type_dist2_later n) T.
+  Proof. intros Hf [|n]; last exact: Hf. hnf. by intros. Qed.
+
+  (* From the above, it easily follows that TypeNonExpansive functions compose with
+     TypeNonExpansive and with TypeContractive functions. *)
+  Lemma type_ne_ne_compose (T1 : type rt2 → type rt3) (T2 : type rt1 → type rt2) :
+    TypeNonExpansive T1 → TypeNonExpansive T2 → TypeNonExpansive (T1 ∘ T2).
+  Proof. intros NE1 NE2 ? ???; simpl. apply: NE1. exact: NE2. Qed.
+
+  Lemma type_contractive_compose_right (T1 : type rt2 → type rt3) (T2 : type rt1 → type rt2) :
+    TypeContractive T1 → TypeNonExpansive T2 → TypeContractive (T1 ∘ T2).
+  Proof. intros HT1 HT2 ? ???. apply: HT1. exact: type_ne_dist_later. Qed.
+
+  Lemma type_contractive_compose_left (T1 : type rt2 → type rt3) (T2 : type rt1 → type rt2) :
+    TypeNonExpansive T1 → TypeContractive T2 → TypeContractive (T1 ∘ T2).
+  Proof. intros HT1 HT2 ? ???; simpl. apply: HT1. exact: HT2. Qed.
+
+  (* Show some more relationships between properties. *)
+  Lemma type_contractive_type_ne (T : type rt1 → type rt2) :
+    TypeContractive T → TypeNonExpansive T.
+  Proof.
+    intros HT ? ???.
+    (*eapply type_dist_dist2, dist_later_S. type_dist2_dist_later, HT. done.*)
+  (*Qed.*)
+  Admitted.
+
+  Lemma type_contractive_ne (T : type rt1 → type rt2) :
+    TypeContractive T → NonExpansive T.
+  Proof.
+    (*intros HT ? ???. apply dist_later_S, type_dist2_dist_later, HT, type_dist_dist2. done.*)
+  (*Qed.*)
+  Abort.
+
+  (* Simple types *)
+  (*
+  Global Instance ty_of_st_type_ne n :
+    Proper (dist_later n ==> type_dist2 n) ty_of_st.
+  Proof.
+    intros ?? Hdst. constructor.
+    - done.
+    - intros. dist_later_intro. eapply Hdst.
+    - intros. solve_contractive.
+  Qed.
+  *)
+End type_contractive.
+
+(* Tactic automation. *)
+(*
+Ltac f_type_equiv :=
+  first [ ((eapply ty_size_type_dist || eapply ty_shr_type_dist || eapply ty_own_type_dist); try reflexivity) |
+          match goal with | |- @dist_later ?A _ ?n ?x ?y =>
+                            eapply dist_later_fin_iff; destruct n as [|n]; [exact I|change (@dist A _ n x y)]
+          end ].
+Ltac solve_type_proper :=
+  constructor;
+  solve_proper_core ltac:(fun _ => f_type_equiv || f_contractive_fin || f_equiv).
+  *)
