theories/rust_typing/fixpoint.v
@@ -1,0 +1,11 @@
+From refinedrust Require Import type.
+From iris.prelude Require Import options.
+
+Section fixpoint_def.
+  Context `{!typeGS Σ}.
+
+  Context {T_rt : Type} (T : type T_rt → type T_rt) {HT : TypeContractive T}.
+
+  Axiom fixpoint_t : type T_rt.
+
+End fixpoint_def.
