theories/rust_typing/shr_ref.v
@@ -1,0 +1,1492 @@
+From caesium Require Import derived.
+From refinedrust Require Export base type ltypes.
+From refinedrust Require Import programs ltype_rules.
+
+Local Definition ref_layout := void_ptr.
+
+(** * Shared references *)
+Section shr_ref.
+  Context `{typeGS Σ} {rt} (inner : type rt).
+  Implicit Types (κ : lft).
+
+  (* this is almost a simple type, but we have to be careful with
+    the sharing predicate: we want to obtain the knowledge that l points to
+    a location not under a later (to prove the agreement with the ltype unfolding),
+     so the simple_type interface doesn't suffice *)
+  Program Definition shr_ref κ : type (place_rfn rt) := {|
+    ty_sidecond := True;
+    ty_own_val π r v :=
+      (∃ (l : loc) (ly : layout) (r' : rt),
+        ⌜v = val_of_loc l⌝ ∗
+        ⌜use_layout_alg inner.(ty_syn_type) = Some ly⌝ ∗ ⌜l `has_layout_loc` ly⌝ ∗
+        loc_in_bounds l 0 ly.(ly_size) ∗
+        inner.(ty_sidecond) ∗
+        place_rfn_interp_shared r r' ∗
+        □ |={lftE}=> inner.(ty_shr) κ π r' l)%I;
+
+    _ty_has_op_type ot mt := is_ptr_ot ot;
+    ty_syn_type := PtrSynType;
+
+    ty_shr κ' π r l :=
+      (∃ (li : loc) (ly : layout) (ri : rt),
+        ⌜l `has_layout_loc` void*⌝ ∗
+        (*loc_in_bounds l void*.(ly_size) ∗*)
+        ⌜use_layout_alg inner.(ty_syn_type) = Some ly⌝ ∗
+        ⌜li `has_layout_loc` ly⌝ ∗
+        loc_in_bounds li 0 ly.(ly_size) ∗
+        inner.(ty_sidecond) ∗
+        place_rfn_interp_shared r ri ∗
+        &frac{κ'} (λ q, l ↦{q} li) ∗ ▷ □ |={lftE}=> inner.(ty_shr) (κ) π ri li)%I;
+    ty_ghost_drop _ _ := True%I;
+    ty_lfts := κ :: inner.(ty_lfts);
+    ty_wf_E := ty_outlives_E inner κ;
+  |}.
+  Next Obligation. iIntros (????) "(%l & %ly & %r' & -> & ? & ? & ?)". eauto. Qed.
+  Next Obligation.
+    iIntros (? ot Hot) => /=. destruct ot => /=// -> //.
+  Qed.
+  Next Obligation. iIntros (????) "_". done. Qed.
+  Next Obligation. iIntros (?????) "_". done. Qed.
+  Next Obligation.
+    iIntros (?????). simpl. iIntros "(%l' & %ly & %r' & ? & ? & ? & _)". eauto.
+  Qed.
+  Next Obligation.
+    iIntros (κ E κ' l ly π r q ?) "#[LFT TIME] Htok %Halg %Hly _ Hb".
+    simpl. rewrite -{1}lft_tok_sep -{1}lft_tok_sep.
+    iDestruct "Htok" as "(Htok_κ' & Htok_κ & Htok)".
+    iApply fupd_logical_step.
+    iMod (bor_exists with "LFT Hb") as "(%v & Hb)"; first solve_ndisj.
+    iMod (bor_sep with "LFT Hb") as "[Hl Hb]"; first solve_ndisj.
+    iMod (bor_exists with "LFT Hb") as "(%l' & Hb)"; first solve_ndisj.
+    iMod (bor_exists with "LFT Hb") as "(%ly' & Hb)"; first solve_ndisj.
+    iMod (bor_exists_tok with "LFT Hb Htok_κ'") as "(%r' & Hb & Htok_κ')"; first solve_ndisj.
+    iMod (bor_sep with "LFT Hb") as "(Heq & Hb)"; first solve_ndisj.
+    iMod (bor_persistent with "LFT Heq Htok_κ'") as "(>-> & Htok_κ')"; first solve_ndisj.
+    iMod (bor_persistent with "LFT Hb Htok_κ'") as "(Ha & Htok_κ')"; first solve_ndisj.
+    iDestruct "Ha" as "(>%Halg' & >%Hly' & >#Hlb & >#Hsc & >Hrfn & Hshr)".
+    iMod (bor_fracture (λ q, l ↦{q} l')%I with "LFT Hl") as "Hl"; first solve_ndisj.
+    iModIntro.
+    iApply logical_step_intro.
+    rewrite -!lft_tok_sep. iFrame.
+    iExists l', ly', r'.
+    iSplitR. { inversion Halg; subst; done. }
+    iSplitR; first done. iSplitR; first done.
+    iSplitR; first done. iSplitR; first done.
+    iFrame.
+  Qed.
+  Next Obligation.
+    iIntros (? κ' κ'' π r l) "#Hord H".
+    iDestruct "H" as (li ly ri) "(? & ? & ? & Hlb & Hsc & Hr & #Hf & #Hown)".
+    iExists li, ly, ri. iFrame. iSplit.
+    - by iApply (frac_bor_shorten with "Hord").
+    - iNext. iDestruct "Hown" as "#Hown". iModIntro. iMod "Hown". iModIntro.
+      done.
+  Qed.
+  Next Obligation.
+    iIntros (??????) "Ha".
+    iApply logical_step_intro. done.
+  Qed.
+  Next Obligation.
+    iIntros (? ot mt st ? r ? Hot).
+    destruct mt.
+    - eauto.
+    - iIntros "(%l & %ly & %ri & -> & ? & ? & ?)".
+      iExists l, ly, ri. iFrame.
+      iPureIntro. move: ot Hot => [] /=// _.
+      rewrite /mem_cast val_to_of_loc //.
+    - iApply (mem_cast_compat_loc (λ v, _)); first done.
+      iIntros "(%l & %ly & %ri & -> & _)". eauto.
+  Qed.
+
+  Global Instance shr_ref_copyable κ : Copyable (shr_ref κ).
+  Proof.
+    constructor; first apply _.
+    iIntros (κ' π E  F l ly r ? ? Ha ?) "[LFT TIME] (%li & %ly' & %r' & %Hly' & % & % & #Hlb & #Hsc & #Hr & Hf & #Hown) Htok Hlft".
+    iDestruct (na_own_acc with "Htok") as "[$ Htok]"; first solve_ndisj.
+    iMod (frac_bor_acc with "LFT Hf Hlft") as (q') "[Hmt Hclose]"; first solve_ndisj.
+    iModIntro.
+    assert (ly = void*) as ->. { injection Ha. done. }
+    iSplitR; first done.
+    iExists _, li. iDestruct "Hmt" as "[Hmt1 Hmt2]".
+    iSplitL "Hmt1". { iNext. iFrame "Hmt1". iExists li, ly', r'. iFrame "#". eauto. }
+    iIntros "Htok2 Hmt1".
+    iDestruct ("Htok" with "Htok2") as "$".
+    iApply "Hclose". iModIntro. rewrite -{3}(Qp.div_2 q').
+    iPoseProof (heap_mapsto_agree with "Hmt1 Hmt2") as "%Heq"; first done.
+    rewrite heap_mapsto_fractional. iFrame.
+  Qed.
+End shr_ref.
+
+Section ofty.
+  Context `{!typeGS Σ}.
+
+  (** A very fundamental equivalence that should hold *)
+  Lemma shr_ref_ofty_shared_equiv {rt} (ty : type rt) π κ l r :
+    l ◁ₗ[π, Shared κ] #r @ (◁ ty) ⊣⊢ l ◁ᵥ{π} #r @ shr_ref ty κ.
+  Proof.
+    rewrite ltype_own_ofty_unfold/lty_of_ty_own /ty_own_val/=.
+    iSplit.
+    - iIntros "(%ly & %Hst & %Hly & #Hsc & #Hlb & %r' & <- & #Ha)".
+      iExists _, _, _. iR. iR. iR. iFrame "#". done.
+    -iIntros "(%l' & %ly & %r' & %Hl & % & % & #Hsc & #Hlb & <- & #Ha)".
+      apply val_of_loc_inj in Hl. subst.
+      iExists _. iR. iR. iFrame "#". iExists _. iR. done.
+  Qed.
+End ofty.
+
+Section subtype.
+  Context `{typeGS Σ}.
+
+  Lemma shr_ref_own_val_mono_in {rt1 rt2} (ty1 : type rt1) (ty2 : type rt2) v π r1 r2 κ1 κ2 :
+    κ1 ⊑ κ2 -∗
+    type_incl r1 r2 ty1 ty2 -∗
+    v ◁ᵥ{π} #r1 @ shr_ref ty1 κ2 -∗
+    v ◁ᵥ{π} #r2 @ shr_ref ty2 κ1.
+  Proof.
+    iIntros "#Hincl (%Hst_eq & #Hsc_eq & _ & #Hincl_shr)".
+    iIntros "(%l & %ly & %r' & -> & ? & ? & Hlb & Hsc & -> & #Hl)". iExists l, ly, r2.
+    iSplitR; first done. rewrite -Hst_eq. iFrame.
+    iSplitL "Hsc". { by iApply "Hsc_eq". }
+    iR. iModIntro. iMod "Hl". iModIntro.
+    iApply ty_shr_mono; first iApply "Hincl".
+    by iApply "Hincl_shr".
+  Qed.
+  Lemma shr_ref_own_val_mono {rt} `{!Inhabited rt} (ty1 ty2 : type rt) v π r κ1 κ2 :
+    κ1 ⊑ κ2 -∗
+    (∀ r, type_incl r r ty1 ty2) -∗
+    v ◁ᵥ{π} r @ shr_ref ty1 κ2 -∗
+    v ◁ᵥ{π} r @ shr_ref ty2 κ1.
+  Proof.
+    iIntros "#Hincl #Hsub".
+    iDestruct ("Hsub" $! inhabitant) as "(%Hst_eq & #Hsc_eq & _)".
+    iIntros "(%l & %ly & %r' & -> & ? & ? & Hlb & Hsc & Hr & #Hl)". iExists l, ly, r'.
+    iSplitR; first done. rewrite -Hst_eq. iFrame.
+    iSplitL "Hsc". { by iApply "Hsc_eq". }
+    iModIntro. iMod "Hl". iModIntro.
+    iPoseProof ("Hsub" $! r') as "(_ & _ & _ & #Hincl_shr)".
+    iApply ty_shr_mono; first iApply "Hincl".
+    by iApply "Hincl_shr".
+  Qed.
+
+  Lemma shr_ref_shr_mono_in {rt1 rt2} (ty1 : type rt1) (ty2 : type rt2) l π κ r1 r2 κ1 κ2 :
+    κ1 ⊑ κ2 -∗
+    type_incl r1 r2 ty1 ty2 -∗
+    l ◁ₗ{π, κ} #r1 @ shr_ref ty1 κ2 -∗
+    l ◁ₗ{π, κ} #r2 @ shr_ref ty2 κ1.
+  Proof.
+    iIntros "#Hincl (%Hst_eq & #Hsc_eq & _ & #Hincl_shr)".
+    iIntros "(%li & %ly & %r' & ? & ? & ? & Hlb & Hsc & -> & Hli & #Hb)".
+    iExists li, ly, r2. rewrite Hst_eq. iFrame.
+    iSplitL "Hsc". { by iApply "Hsc_eq". }
+    iR. iModIntro. iDestruct "Hb" as "#Hb". iModIntro. iMod "Hb". iModIntro.
+    iApply ty_shr_mono; first iApply "Hincl".
+    by iApply "Hincl_shr".
+  Qed.
+  Lemma shr_ref_shr_mono {rt} `{!Inhabited rt} (ty1 ty2 : type rt) l π κ r κ1 κ2 :
+    κ1 ⊑ κ2 -∗
+    (∀ r, type_incl r r ty1 ty2) -∗
+    l ◁ₗ{π, κ} r @ shr_ref ty1 κ2 -∗
+    l ◁ₗ{π, κ} r @ shr_ref ty2 κ1.
+  Proof.
+    iIntros "#Hincl #Hsub".
+    iPoseProof ("Hsub" $! inhabitant) as "(%Hst_eq & #Hsc_eq & _)".
+    iIntros "(%li & %ly & %r' & ? & ? & ? & Hlb & Hsc & Hr & Hli & #Hb)".
+    iExists li, ly, r'. rewrite Hst_eq. iFrame.
+    iSplitL "Hsc". { by iApply "Hsc_eq". }
+    iModIntro. iDestruct "Hb" as "#Hb". iModIntro. iMod "Hb". iModIntro.
+    iPoseProof ("Hsub" $! r') as "(_ & _ & _ & #Hincl_shr)".
+    iApply ty_shr_mono; first iApply "Hincl".
+    by iApply "Hincl_shr".
+  Qed.
+
+  Lemma shr_ref_type_incl_in {rt1 rt2} κ2 κ1 (ty1 : type rt1) (ty2 : type rt2) r1 r2 :
+    κ1 ⊑ κ2 -∗
+    type_incl r1 r2 ty2 ty1 -∗
+    type_incl #r1 #r2 (shr_ref ty2 κ2) (shr_ref ty1 κ1).
+  Proof.
+    iIntros "#Hincl #Hsub".
+    iSplitR; first done. iSplitR; first done.
+    iSplit; iIntros "!#".
+    - iIntros (??). by iApply shr_ref_own_val_mono_in.
+    - iIntros (???). by iApply shr_ref_shr_mono_in.
+  Qed.
+  Lemma shr_ref_type_incl {rt} `{!Inhabited rt} κ2 κ1 (ty1 ty2 : type rt) r :
+    κ1 ⊑ κ2 -∗
+    (∀ r, type_incl r r ty2 ty1) -∗
+    type_incl r r (shr_ref ty2 κ2) (shr_ref ty1 κ1).
+  Proof.
+    iIntros "#Hincl #Hsub".
+    iSplitR; first done. iSplitR; first done.
+    iSplit; iIntros "!#".
+    - iIntros (??). by unshelve iApply shr_ref_own_val_mono.
+    - iIntros (???). by unshelve iApply shr_ref_shr_mono.
+  Qed.
+
+  Lemma shr_ref_full_subtype {rt} `{!Inhabited rt} E L κ2 κ1 (ty1 ty2 : type rt) :
+    lctx_lft_incl E L κ1 κ2 →
+    full_subtype E L ty2 ty1 →
+    full_subtype E L (shr_ref ty2 κ2) (shr_ref ty1 κ1).
+  Proof.
+    iIntros (Hincl Hsubt r ?) "HL #HE".
+    iPoseProof (Hincl with "HL") as "#Hincl".
+    iSpecialize ("Hincl" with "HE").
+    iPoseProof (full_subtype_acc_noend with "HE HL") as "#Hsubt"; first apply Hsubt.
+    unshelve iApply shr_ref_type_incl; done.
+  Qed.
+End subtype.
+
+
+Section subltype.
+  Context `{!typeGS Σ}.
+
+  (** Shared references *)
+  Local Lemma shr_ltype_incl'_shared_in {rt1 rt2} (lt1 : ltype rt1) (lt2 : ltype rt2) κ' r1 r2 κ1 κ2 :
+    ltype_incl (Shared (κ1)) r1 r2 lt1 lt2 -∗
+    κ2 ⊑ κ1 -∗
+    ltype_incl' (Shared κ') #(r1) #(r2) (ShrLtype lt1 κ1) (ShrLtype lt2 κ2).
+  Proof.
+    iIntros "#Heq #Hincl1".
+    iModIntro.
+    iIntros (π l). rewrite !ltype_own_shr_ref_unfold /shr_ltype_own.
+    iIntros "(%ly & ? & ? & Hlb & %ri & Hrfn & #Hb)".
+    iExists ly. iFrame. rewrite -?Hd -?Hly_eq. iFrame.
+    iDestruct "Hrfn" as "->".
+    iExists r2. iSplitR; first done. iModIntro. iMod "Hb".
+    iDestruct "Hb" as "(%li & Hs & Hb)". iModIntro. iExists li. iFrame. iNext.
+    iDestruct "Heq" as "(_ & Hi1 & _)".
+    iApply ltype_own_shr_mono; last by iApply "Hi1". done.
+  Qed.
+  Lemma shr_ltype_incl_shared_in {rt1 rt2} (lt1 : ltype rt1) (lt2 : ltype rt2) κ' r1 r2 κ1 κ2 :
+    ltype_incl (Shared (κ1)) r1 r2 lt1 lt2 -∗
+    κ2 ⊑ κ1 -∗
+    ltype_incl (Shared κ') #(r1) #(r2) (ShrLtype lt1 κ1) (ShrLtype lt2 κ2).
+  Proof.
+    iIntros "#Heq #Hincl1".
+    iPoseProof (ltype_incl_syn_type with "Heq") as "%Hst".
+    iSplitR; first done. iModIntro.
+    simp_ltypes.
+    iSplit; (iApply shr_ltype_incl'_shared_in; [ | done  ]).
+    - done.
+    - iApply ltype_incl_core. done.
+  Qed.
+
+  Local Lemma shr_ltype_incl'_shared {rt} (lt1 lt2 : ltype rt) κ' r κ1 κ2 :
+    (∀ r, ltype_incl (Shared (κ1)) r r lt1 lt2) -∗
+    κ2 ⊑ κ1 -∗
+    ltype_incl' (Shared κ') r r (ShrLtype lt1 κ1) (ShrLtype lt2 κ2).
+  Proof.
+    iIntros "#Heq #Hincl1".
+    iModIntro.
+    iIntros (π l). rewrite !ltype_own_shr_ref_unfold /shr_ltype_own.
+    iIntros "(%ly & ? & ? & Hlb & %ri & Hrfn & #Hb)".
+    iExists ly. iFrame. rewrite -?Hd -?Hly_eq. iFrame.
+    iExists ri. iFrame. iModIntro. iMod "Hb".
+    iDestruct "Hb" as "(%li & Hs & Hb)". iModIntro. iExists li. iFrame. iNext.
+    iDestruct ("Heq" $! _) as "(_ & Hi1 & _)".
+    iApply ltype_own_shr_mono; last by iApply "Hi1". done.
+  Qed.
+  Lemma shr_ltype_incl_shared {rt} (lt1 : ltype rt) (lt2 : ltype rt) κ' r κ1 κ2 :
+    (∀ r, ltype_incl (Shared (κ1)) r r lt1 lt2) -∗
+    κ2 ⊑ κ1 -∗
+    ltype_incl (Shared κ') r r (ShrLtype lt1 κ1) (ShrLtype lt2 κ2).
+  Proof.
+    iIntros "#Heq #Hincl1".
+    iPoseProof (ltype_incl_syn_type _ inhabitant with "Heq") as "%Hst".
+    iSplitR; first done. iModIntro.
+    simp_ltypes.
+    iSplit; (iApply shr_ltype_incl'_shared; [ | done  ]).
+    - done.
+    - iIntros (?). iApply ltype_incl_core. done.
+  Qed.
+
+  Local Lemma shr_ltype_incl'_owned_in {rt1 rt2} (lt1 : ltype rt1) (lt2 : ltype rt2) κ1 κ2 wl r1 r2 :
+    ltype_incl (Shared κ1) r1 r2 lt1 lt2  -∗
+    κ2 ⊑ κ1 -∗
+    ltype_incl' (Owned wl) #(r1) #(r2) (ShrLtype lt1 κ1) (ShrLtype lt2 κ2).
+  Proof.
+    iIntros "#Heq #Hincl1". iModIntro.
+    iIntros (π l). rewrite !ltype_own_shr_ref_unfold /shr_ltype_own.
+    iIntros "(%ly & ? & ? & Hlb & ? & %ri & Hrfn & Hb)".
+    iModIntro.
+    iExists ly. iFrame. rewrite -?Hd -?Hly_eq.
+    iFrame. iDestruct "Hrfn" as "->". iExists r2. iSplitR; first done. iNext.
+    iMod "Hb" as "(%li & Hli & Hb)". iExists li. iFrame "Hli".
+    iDestruct "Heq" as "(_ & Heq & _)".
+    iApply ltype_own_shr_mono; last by iApply "Heq". done.
+  Qed.
+  Lemma shr_ltype_incl_owned_in {rt1 rt2} (lt1 : ltype rt1) (lt2 : ltype rt2) κ1 κ2 wl r1 r2 :
+    ltype_incl (Shared κ1) r1 r2 lt1 lt2  -∗
+    κ2 ⊑ κ1 -∗
+    ltype_incl (Owned wl) #(r1) #(r2) (ShrLtype lt1 κ1) (ShrLtype lt2 κ2).
+  Proof.
+    iIntros "#Heq #Hincl1".
+    iPoseProof (ltype_incl_syn_type with "Heq") as "%Hst".
+    iSplitR; first done. iModIntro.
+    simp_ltypes.
+    iSplit; (iApply shr_ltype_incl'_owned_in; [ | done  ]).
+    - done.
+    - iApply ltype_incl_core. done.
+  Qed.
+
+  Local Lemma shr_ltype_incl'_owned {rt} (lt1 lt2 : ltype rt) κ1 κ2 wl r :
+    (∀ r, ltype_incl (Shared κ1) r r lt1 lt2) -∗
+    κ2 ⊑ κ1 -∗
+    ltype_incl' (Owned wl) r r (ShrLtype lt1 κ1) (ShrLtype lt2 κ2).
+  Proof.
+    iIntros "#Heq #Hincl1". iModIntro.
+    iIntros (π l). rewrite !ltype_own_shr_ref_unfold /shr_ltype_own.
+    iIntros "(%ly & ? & ? & Hlb & ? & %ri & Hrfn & Hb)".
+    iModIntro.
+    iExists ly. iFrame. rewrite -?Hd -?Hly_eq.
+    iFrame. iExists ri. iFrame. iNext.
+    iMod "Hb" as "(%li & Hli & Hb)". iExists li. iFrame "Hli".
+    iDestruct ("Heq" $! _) as "(_ & Heq' & _)".
+    iApply ltype_own_shr_mono; last by iApply "Heq'". done.
+  Qed.
+  Lemma shr_ltype_incl_owned {rt} (lt1 : ltype rt) (lt2 : ltype rt) κ1 κ2 wl r :
+    (∀ r, ltype_incl (Shared κ1) r r lt1 lt2)  -∗
+    κ2 ⊑ κ1 -∗
+    ltype_incl (Owned wl) r r (ShrLtype lt1 κ1) (ShrLtype lt2 κ2).
+  Proof.
+    iIntros "#Heq #Hincl1".
+    iPoseProof (ltype_incl_syn_type (Shared _) inhabitant with "Heq") as "%Hst".
+    iSplitR; first done. iModIntro.
+    simp_ltypes.
+    iSplit; (iApply shr_ltype_incl'_owned; [ | done  ]).
+    - done.
+    - iIntros (?). iApply ltype_incl_core. done.
+  Qed.
+
+  (* Refinement subtyping under mutable references is restricted: we need to make sure that, no matter the future updates,
+     we can always get back to what the lender expects. Thus we loose all refinement information when descending below mutable references. *)
+  Local Lemma shr_ltype_incl'_uniq {rt} (lt1 lt2 : ltype rt) κ1 κ2 κ r γ :
+    (∀ r, ltype_eq (Shared (κ1)) r r lt1 lt2) -∗
+    (* Note: requires mutual inclusion, because we may be below a mutable reference *)
+    κ2 ⊑ κ1 -∗
+    κ1 ⊑ κ2 -∗
+    ltype_incl' (Uniq κ γ) r r (ShrLtype lt1 κ1) (ShrLtype lt2 κ2).
+  Proof.
+    iIntros "#Heq #Hincl1 #Hincl2". iModIntro.
+    iIntros (π l). rewrite !ltype_own_shr_ref_unfold /shr_ltype_own.
+    iIntros "(%ly & ? & ? & Hlb & ? &  Hrfn & Hb)".
+    iExists ly. iFrame. rewrite -?Hly_eq. iFrame.
+    iMod "Hb". iModIntro. iApply (pinned_bor_iff with "[] [] Hb").
+    + iNext. iModIntro. iSplit.
+      * iIntros "(%ri & Hauth & Hb)". iExists ri. iFrame.
+        iMod "Hb" as "(%li & Hl & Hb)". iModIntro. iExists _. iFrame.
+        iDestruct ("Heq" $! ri) as "((_ & Hi & _) & _)".
+        iApply ltype_own_shr_mono; last by iApply "Hi". done.
+      * iIntros "(%ri & Hauth & Hb)". iExists ri. iFrame.
+        iMod "Hb" as "(%li & Hl & Hb)". iModIntro. iExists _. iFrame.
+        iDestruct ("Heq" $! ri) as "(_ & (_ & Hi & _))".
+        iApply "Hi"; last by iApply ltype_own_shr_mono.
+    + (* the same proof *)
+      iNext. iModIntro. iSplit.
+      * iIntros "(%ri & Hauth & Hb)". iExists ri. iFrame.
+        iMod "Hb" as "(%li & Hl & Hb)". iModIntro. iExists _. iFrame.
+        iDestruct ("Heq" $! ri) as "((_ & _ & Hi) & _)".
+        rewrite !ltype_own_core_equiv.
+        iApply ltype_own_shr_mono; last by iApply "Hi". done.
+      * iIntros "(%ri & Hauth & Hb)". iExists ri. iFrame.
+        iMod "Hb" as "(%li & Hl & Hb)". iModIntro. iExists _. iFrame.
+        iDestruct ("Heq" $! ri) as "(_ & (_ & _ & Hi))".
+        rewrite !ltype_own_core_equiv.
+        iApply "Hi"; last by iApply ltype_own_shr_mono.
+  Qed.
+  Lemma shr_ltype_incl_uniq {rt} (lt1 lt2 : ltype rt) κ1 κ2 κ r γ :
+    (∀ r, ltype_eq (Shared (κ1)) r r lt1 lt2) -∗
+    κ2 ⊑ κ1 -∗
+    κ1 ⊑ κ2 -∗
+    ltype_incl (Uniq κ γ) r r (ShrLtype lt1 κ1) (ShrLtype lt2 κ2).
+  Proof.
+    iIntros "#Heq #Hincl1 #Hincl2".
+    iPoseProof (ltype_eq_syn_type _ inhabitant with "Heq") as "%Hst".
+    iSplitR; first done. iModIntro.
+    simp_ltypes.
+    iSplit; (iApply shr_ltype_incl'_uniq; [ | done  | done]).
+    - done.
+    - iIntros (?). iApply ltype_eq_core. done.
+  Qed.
+
+  Lemma shr_ltype_incl {rt} (lt1 lt2 : ltype rt) b r κ1 κ2 :
+    (∀ b r, ltype_eq b r r lt1 lt2) -∗
+    κ2 ⊑ κ1 -∗
+    κ1 ⊑ κ2 -∗
+    ltype_incl b r r (ShrLtype lt1 κ1) (ShrLtype lt2 κ2).
+  Proof.
+    iIntros "#Heq #Hincl1 #Hincl2".
+    destruct b.
+    - iApply shr_ltype_incl_owned; last done. iIntros (?). iDestruct ("Heq" $! _ _) as "[$ _]".
+    - iApply shr_ltype_incl_shared; last done. iIntros (?). iDestruct ("Heq" $! _ _) as "[$ _]".
+    - iApply shr_ltype_incl_uniq; [ | done..]. iIntros (?). done.
+  Qed.
+  Lemma shr_ltype_eq {rt} (lt1 lt2 : ltype rt) b r κ1 κ2 :
+    (∀ b r, ltype_eq b r r lt1 lt2) -∗
+    κ2 ⊑ κ1 -∗
+    κ1 ⊑ κ2 -∗
+    ltype_eq b r r (ShrLtype lt1 κ1) (ShrLtype lt2 κ2).
+  Proof.
+    iIntros "#Heq #Hincl1 #Hincl2".
+    iSplit.
+    - iApply shr_ltype_incl; done.
+    - iApply shr_ltype_incl; [ | done..]. iIntros (??). iApply ltype_eq_sym. done.
+  Qed.
+
+  Lemma shr_full_subltype E L {rt} (lt1 lt2 : ltype rt) κ1 κ2 :
+    full_eqltype E L lt1 lt2 →
+    lctx_lft_incl E L κ1 κ2 →
+    lctx_lft_incl E L κ2 κ1 →
+    full_subltype E L (ShrLtype lt1 κ1) (ShrLtype lt2 κ2).
+  Proof.
+    intros Hsub Hincl1 Hincl2.
+    iIntros (qL) "HL #CTX #HE". iIntros (??).
+    iPoseProof (lctx_lft_incl_incl_noend with "HL HE") as "#Hincl1"; first apply Hincl1.
+    iPoseProof (lctx_lft_incl_incl_noend with "HL HE") as "#Hincl2"; first apply Hincl2.
+    iPoseProof (Hsub  with "HL CTX HE") as "Hsub".
+    iApply (shr_ltype_incl with "Hsub Hincl2 Hincl1").
+  Qed.
+  Lemma shr_full_eqltype E L {rt} (lt1 lt2 : ltype rt) κ1 κ2 :
+    full_eqltype E L lt1 lt2 →
+    lctx_lft_incl E L κ1 κ2 →
+    lctx_lft_incl E L κ2 κ1 →
+    full_eqltype E L (ShrLtype lt1 κ1) (ShrLtype lt2 κ2).
+  Proof.
+    intros Hsub Hincl1 Hincl2.
+    apply full_subltype_eqltype; eapply shr_full_subltype; naive_solver.
+  Qed.
+End subltype.
+
+Section ltype_agree.
+  Context `{typeGS Σ}
+    {rt}
+    (ty : type rt).
+
+  Lemma shr_ref_unfold_1_owned κ wl r :
+    ⊢ ltype_incl' (Owned wl) r r (ShrLtype (◁ ty) κ) (◁ (shr_ref ty κ)).
+  Proof.
+    iModIntro. iIntros (π l). rewrite ltype_own_shr_ref_unfold /shr_ltype_own ltype_own_ofty_unfold /lty_of_ty_own.
+    iIntros "(%ly & ? & ? & #Hlb & ? &  %ri & Hrfn & Hb)".
+    iModIntro.
+    iExists ly.
+    iFrame. iFrame "Hlb". iExists _. iFrame. iNext. iMod "Hb" as "(%l' & Hl & Hb)".
+    rewrite ltype_own_ofty_unfold /lty_of_ty_own.
+    iDestruct "Hb" as "(%ly' & ? & ? & Hsc & Hlb' & %ri' & Hrfn' & Hb)".
+    iExists l'. iFrame. iExists l', _, _. iFrame. done.
+  Qed.
+  Lemma shr_ref_unfold_1_shared `{!Inhabited rt} κ κ' r :
+    ⊢ ltype_incl' (Shared κ') r r (ShrLtype (◁ ty) κ) (◁ (shr_ref ty κ)).
+  Proof.
+    iModIntro. iIntros (π l). rewrite ltype_own_shr_ref_unfold /shr_ltype_own ltype_own_ofty_unfold /lty_of_ty_own.
+    iIntros "(%ly & %Ha & % & #Hlb & %ri & Hrfn & #Hb)".
+    iExists ly. iFrame. iFrame "Hlb %". iExists _. iFrame.
+    iModIntro. iMod "Hb".
+    iDestruct "Hb" as "(%li & #Hs & Hb)".
+    rewrite ltype_own_ofty_unfold /lty_of_ty_own.
+    iDestruct "Hb" as "(%ly' & >? & >? & >Hsc & >Hlb' & %r' & >Hrfn & Hb)". iModIntro.
+    iExists _, _, _. iFrame. iSplitR; last done.
+    injection Ha as <-. done.
+  Qed.
+  Lemma shr_ref_unfold_1_uniq κ κ' γ r :
+    ⊢ ltype_incl' (Uniq κ' γ) r r (ShrLtype (◁ ty) κ) (◁ (shr_ref ty κ)).
+  Proof.
+    iModIntro. iIntros (π l). rewrite ltype_own_shr_ref_unfold /shr_ltype_own ltype_own_ofty_unfold /lty_of_ty_own.
+    iIntros "(%ly & ? & ? & ? & ? & ?  & Hb)". iExists ly. iFrame. iMod "Hb". iModIntro.
+    iApply (pinned_bor_iff with "[] [] Hb").
+    - iNext. iModIntro. iSplit.
+      * iIntros "(%r' & Hauth & Hb)". iExists _. iFrame.
+        iMod "Hb" as "(%l' & Hl & Hb)". iExists l'. iFrame.
+        rewrite ltype_own_ofty_unfold /lty_of_ty_own.
+        iDestruct "Hb" as "(%ly' & ? & ? & Hsc & Hlb & %ri & Hrfn & Hb)".
+        iExists l', ly', _. iFrame. done.
+      * iIntros "(%r' & Hauth & Hb)". iExists _; iFrame.
+        iMod "Hb" as "(%v & Hl & Hb)".
+        iDestruct "Hb" as "(%li & %ly' & %ri & -> & ? & ? & Hlb & Hsc & Hrfn & Hb)".
+        iExists _. iFrame. rewrite ltype_own_ofty_unfold /lty_of_ty_own.
+        iFrame. iExists ly'. iFrame.
+        iExists _. by iFrame.
+    - iNext. iModIntro. iSplit.
+      * iIntros "(%r' & Hauth & Hb)". iExists _. iFrame.
+        iMod "Hb" as "(%l' & Hl & Hb)". iExists l'. iFrame.
+        rewrite ltype_own_core_equiv. simp_ltypes.
+        rewrite ltype_own_ofty_unfold /lty_of_ty_own.
+        iDestruct "Hb" as "(%ly' & ? & ? & Hsc & Hlb & %ri & Hrfn & Hb)".
+        iExists l', ly', _. iFrame. done.
+      * iIntros "(%r' & Hauth & Hb)". iExists _; iFrame.
+        iMod "Hb" as "(%v & Hl & Hb)".
+        iDestruct "Hb" as "(%li & %ly' & %ri & -> & ? & ? & Hlb & Hsc & Hrfn & Hb)".
+        iExists _. iFrame.
+        rewrite ltype_own_core_equiv. simp_ltype.
+        rewrite ltype_own_ofty_unfold /lty_of_ty_own.
+        iFrame. iExists ly'. iFrame.
+        iExists _. by iFrame.
+  Qed.
+
+  Local Lemma shr_ref_unfold_1' `{!Inhabited rt} κ k r :
+    ⊢ ltype_incl' k r r (ShrLtype (◁ ty) κ) (◁ (shr_ref ty κ)).
+  Proof.
+    iModIntro. destruct k.
+    - iApply shr_ref_unfold_1_owned.
+    - iApply shr_ref_unfold_1_shared.
+    - iApply shr_ref_unfold_1_uniq.
+  Qed.
+  Lemma shr_ref_unfold_1 `{!Inhabited rt} κ k r :
+    ⊢ ltype_incl k r r (ShrLtype (◁ ty) κ) (◁ (shr_ref ty κ)).
+  Proof.
+    iSplitR; first done. iModIntro. iSplit.
+    - iApply shr_ref_unfold_1'.
+    - simp_ltypes. iApply shr_ref_unfold_1'.
+  Qed.
+
+  Lemma shr_ref_unfold_2_owned κ wl r :
+    ⊢ ltype_incl' (Owned wl) r r (◁ (shr_ref ty κ)) (ShrLtype (◁ ty) κ).
+  Proof.
+    iModIntro. iIntros (π l). rewrite ltype_own_shr_ref_unfold /shr_ltype_own ltype_own_ofty_unfold /lty_of_ty_own.
+    iIntros "(%ly & ? & ? & Hsc & Hlb & ? & %r' & Hrfn & Hb)".
+    iModIntro. iExists ly. iFrame. iExists _. iFrame.
+    iNext. iMod "Hb" as "(%v & Hl & %li & %ly' & %ri & -> & ? & ? & Hlb' & Hsc' & Hrfn' & Hb)".
+    iExists _. iFrame. rewrite ltype_own_ofty_unfold /lty_of_ty_own.
+    iExists ly'. iFrame.
+    iExists _. by iFrame.
+  Qed.
+  Lemma shr_ref_unfold_2_shared κ κ' r :
+    ⊢ ltype_incl' (Shared κ') r r (◁ (shr_ref ty κ)) (ShrLtype (◁ ty) κ).
+  Proof.
+    iModIntro. iIntros (π l). rewrite ltype_own_shr_ref_unfold /shr_ltype_own ltype_own_ofty_unfold /lty_of_ty_own.
+    iIntros "(%ly & ? & ? & Hsc & Hlb & %r' & Hrfn & #Hb)". iExists ly. iFrame.
+    iExists r'. iFrame. iModIntro. iMod "Hb".
+    iDestruct "Hb" as "(%li & %ly' & %ri & ? & ? & ? & Hlb' & Hsc & Hrfn & Hs & Hb)".
+    iModIntro. iExists _. iFrame. iNext. iDestruct "Hb" as "#Hb".
+    rewrite ltype_own_ofty_unfold /lty_of_ty_own.
+    iExists ly'. iFrame.
+    iExists _. iFrame. done.
+  Qed.
+  Lemma shr_ref_unfold_2_uniq κ κ' γ r :
+    ⊢ ltype_incl' (Uniq κ' γ) r r (◁ (shr_ref ty κ)) (ShrLtype (◁ ty) κ).
+  Proof.
+    iModIntro. iIntros (π l). rewrite ltype_own_shr_ref_unfold /shr_ltype_own ltype_own_ofty_unfold /lty_of_ty_own.
+    (* same proof as above essentially *)
+    iIntros "(%ly & ? & ? & Hsc & ? & ? & ? & Hb)". iExists ly. iFrame. iMod "Hb". iModIntro.
+    iApply (pinned_bor_iff with "[] [] Hb").
+    - iNext. iModIntro. iSplit.
+      * iIntros "(%r' & Hauth & Hb)". iExists _. iFrame.
+        iMod "Hb" as "(%v & Hl & Hb)".
+        iDestruct "Hb" as "(%li & %ly' & %ri & -> & ? & ? & Hlb & Hsc & Hrfn & Hb)".
+        iExists _. iFrame. rewrite ltype_own_ofty_unfold /lty_of_ty_own.
+        iExists ly'. iFrame.
+        iExists _. by iFrame.
+      * iIntros "(%r' & Hauth & Hb)". iExists _. iFrame.
+        iMod "Hb" as "(%l' & Hl & Hb)".
+        iExists l'. iFrame. rewrite ltype_own_ofty_unfold /lty_of_ty_own.
+        iDestruct "Hb" as "(%ly' & ? & ? & Hsc & Hlb & %ri & Hrfn & Hb)".
+        iExists l', _, _. iFrame. done.
+    - iNext. iModIntro. iSplit.
+      * iIntros "(%r' & Hauth & Hb)". iExists _. iFrame.
+        iMod "Hb" as "(%v & Hl & Hb)".
+        iDestruct "Hb" as "(%li & %ly' & %ri & -> & ? & ? & Hlb & Hsc & Hrfn & Hb)".
+        iExists _. iFrame. rewrite ltype_own_core_equiv. simp_ltypes.
+        rewrite ltype_own_ofty_unfold /lty_of_ty_own.
+        iExists ly'. iFrame.
+        iExists _. by iFrame.
+      * iIntros "(%r' & Hauth & Hb)". iExists _. iFrame.
+        iMod "Hb" as "(%l' & Hl & Hb)".
+        iExists l'. iFrame. rewrite ltype_own_core_equiv. simp_ltype.
+        rewrite ltype_own_ofty_unfold /lty_of_ty_own.
+        iDestruct "Hb" as "(%ly' & ? & ? & Hsc & Hlb & %ri & Hrfn & Hb)".
+        iExists l', _, _. iFrame. done.
+  Qed.
+
+
+  Local Lemma shr_ref_unfold_2' κ k r :
+    ⊢ ltype_incl' k r r (◁ (shr_ref ty κ)) (ShrLtype (◁ ty) κ).
+  Proof.
+    destruct k.
+    - iApply shr_ref_unfold_2_owned.
+    - iApply shr_ref_unfold_2_shared.
+    - iApply shr_ref_unfold_2_uniq.
+  Qed.
+  Lemma shr_ref_unfold_2 κ k r :
+    ⊢ ltype_incl k r r (◁ (shr_ref ty κ)) (ShrLtype (◁ ty) κ).
+  Proof.
+    iSplitR; first done. iModIntro; iSplit.
+    - iApply shr_ref_unfold_2'.
+    - simp_ltypes. iApply shr_ref_unfold_2'.
+  Qed.
+
+  Lemma shr_ref_unfold `{!Inhabited rt} κ k r :
+    ⊢ ltype_eq k r r (ShrLtype (◁ (ty)) κ) (◁ (shr_ref ty κ)).
+  Proof.
+    iSplit.
+    - iApply shr_ref_unfold_1.
+    - iApply shr_ref_unfold_2.
+  Qed.
+
+  Lemma shr_ref_unfold_full_eqltype `{!Inhabited rt} E L κ (lt : ltype rt) :
+    full_eqltype E L lt (◁ ty)%I →
+    full_eqltype E L (ShrLtype lt κ) (◁ (shr_ref ty κ))%I.
+  Proof.
+    iIntros (Heql ?) "HL #CTX #HE". iIntros (??).
+    iPoseProof (Heql with "HL CTX HE") as "#Heql".
+    iApply ltype_eq_trans; last iApply shr_ref_unfold.
+    iApply shr_ltype_eq; [ | iApply lft_incl_refl.. ].
+    by iApply "Heql".
+  Qed.
+End ltype_agree.
+
+Global Typeclasses Opaque shr_ref.
+Notation "&shr< κ , τ >" := (shr_ref τ κ) (only printing, format "'&shr<' κ , τ '>'") : stdpp_scope.
+
+Section acc.
+  Context `{!typeGS Σ}.
+
+  Lemma shr_ltype_place_cond_ty b κ {rt1 rt2} (lt1 : ltype rt1) (lt2 : ltype rt2) :
+    typed_place_cond_ty b lt1 lt2 -∗
+    typed_place_cond_ty b (ShrLtype lt1 κ) (ShrLtype lt2 κ).
+  Proof.
+    destruct b; simpl.
+    - iIntros "_". done.
+    - iIntros "(-> & %)". simp_ltypes. done.
+    - iIntros "(%Hrefl & Heq & Hub)".
+      subst rt2. cbn.
+      iExists eq_refl. cbn. iSplitR "Hub".
+      + simp_ltypes. iIntros (??). iApply (shr_ltype_eq with "Heq"); iApply lft_incl_refl.
+      + by iApply shr_ltype_imp_unblockable.
+  Qed.
+
+  Lemma shr_ltype_acc_owned {rt} F π (lt : ltype rt) (r : place_rfn rt) l κ' wl :
+    lftE ⊆ F →
+    rrust_ctx -∗
+    l ◁ₗ[π, Owned wl] PlaceIn (r) @ ShrLtype lt κ' -∗
+    ⌜l `has_layout_loc` void*⌝ ∗ loc_in_bounds l 0 (ly_size void*) ∗ |={F}=>
+      ∃ (l' : loc), l ↦ l' ∗ l' ◁ₗ[π, Shared κ'] r @ lt ∗
+      logical_step F
+      (∀ bmin rt' (lt2 : ltype rt') r2,
+        l ↦ l' -∗
+        l' ◁ₗ[π, Shared κ'] r2 @ lt2 ={F}=∗
+        l ◁ₗ[π, Owned wl] PlaceIn (r2) @ ShrLtype lt2 κ' ∗
+        (typed_place_cond bmin lt lt2 r r2 -∗
+         ⌜place_access_rt_rel bmin rt rt'⌝ -∗
+         typed_place_cond bmin (ShrLtype lt κ') (ShrLtype lt2 κ') (PlaceIn (r)) (PlaceIn (r2)))).
+  Proof.
+    iIntros (?) "#[LFT TIME] HP".
+    rewrite ltype_own_shr_ref_unfold /shr_ltype_own.
+    iDestruct "HP" as "(%ly & %Halg & %Hly & #Hlb & Hcred & %r' & %Heq & Hb)".
+    injection Halg as <-. subst.
+    iFrame "Hlb %".
+    iMod (maybe_use_credit with "Hcred Hb") as "(Hcred & Hat & Hb)"; first done.
+    iDestruct "Hb" as "(%l' & Hl & Hb)".
+    iModIntro. iExists l'. iFrame.
+    iApply (logical_step_intro_maybe with "Hat").
+    iIntros "Hcred' !>". iIntros (bmin rt2 lt2 r2) "Hl Hb".
+    iModIntro. iSplitL.
+    - rewrite ltype_own_shr_ref_unfold /shr_ltype_own. iExists void*.
+      iSplitR; first done. iFrame "Hlb % ∗".
+      iExists _. iSplitR; first done. iNext. eauto with iFrame.
+    - iIntros "Hcond %Hrt". iDestruct "Hcond" as "[Hty Hrfn]".
+      subst. iSplit.
+      + by iApply (shr_ltype_place_cond_ty).
+      + destruct bmin; cbn in Hrt; [ done | subst rt2..].
+        all: by iApply (typed_place_cond_rfn_lift _ _ _ (λ r, PlaceIn (r))).
+  Qed.
+
+
+  (* Note: this doesn't allow changing the type below the shared reference *)
+  Lemma shr_ltype_acc_uniq {rt} F π (lt : ltype rt) (r : place_rfn rt) l κ' κ γ q R :
+    lftE ⊆ F →
+    rrust_ctx -∗
+    q.[κ] -∗
+    (q.[κ] ={lftE}=∗ R) -∗
+    l ◁ₗ[π, Uniq κ γ] #r @ ShrLtype lt κ' -∗
+    ⌜l `has_layout_loc` void*⌝ ∗ loc_in_bounds l 0 (ly_size void*) ∗ |={F}=>
+      ∃ l' : loc, l ↦ l' ∗ (l' ◁ₗ[π, Shared κ'] r @ lt) ∗
+      logical_step F
+      ( (* weak update *)
+       (∀ bmin r2,
+        l ↦ l' -∗
+        l' ◁ₗ[π, Shared κ'] r2 @ lt -∗
+        bmin ⊑ₖ Uniq κ γ -∗
+        typed_place_cond bmin lt lt r r2 ={F}=∗
+        l ◁ₗ[π, Uniq κ γ] #r2 @ ShrLtype lt κ' ∗
+        R ∗
+        typed_place_cond bmin (ShrLtype lt κ') (ShrLtype lt κ') (#r) (#r2)) ∧
+      (* strong update, go to Opened *)
+      (∀ rt2 (lt2 : ltype rt2) r2,
+        l ↦ l' -∗
+        ⌜ltype_st lt2 = ltype_st lt⌝ -∗
+        l' ◁ₗ[π, Shared κ'] r2 @ lt2 ={F}=∗
+        l ◁ₗ[π, Uniq κ γ] #r2 @ OpenedLtype (ShrLtype lt2 κ') (ShrLtype lt κ') (ShrLtype lt κ')
+          (λ r1 r1', ⌜r1 = r1'⌝) (λ _ _, R))).
+  Proof.
+    iIntros (?) "#[LFT TIME] Hκ HR HP".
+    rewrite ltype_own_shr_ref_unfold /shr_ltype_own.
+    iDestruct "HP" as "(%ly & %Halg & %Hly & #Hlb & (Hcred & Hat) & Hrfn & Hb)".
+    injection Halg as <-. iFrame "Hlb". iSplitR; first done.
+
+    iMod (fupd_mask_subseteq lftE) as "Hcl_F"; first done.
+    iMod "Hb".
+    (* NOTE: we are currently throwing away the existing "coring"-viewshift that we get *)
+    iMod (pinned_bor_acc_strong lftE with "LFT Hb Hκ") as "(%κ'' & #Hincl & Hb & Hx & Hb_cl)"; first done.
+    iMod "Hcl_F" as "_".
+    iDestruct "Hcred" as "(Hcred1 & Hcred)".
+    iApply (lc_fupd_add_later with "Hcred1"). iNext.
+    iDestruct "Hb" as "(%r' &  Hauth & Hb)".
+    iPoseProof (gvar_agree with "Hauth Hrfn") as "#->".
+    iMod (fupd_mask_mono with "Hb") as "(%l' & Hl & Hb)"; first done.
+    iModIntro. iExists l'. iFrame.
+    iApply (logical_step_intro_atime with "Hat").
+    iIntros "Hcred' Hat".
+    iModIntro.
+    iSplit.
+    - (* close *)
+      iIntros (bmin r2) "Hl Hb #Hincl_k #Hcond".
+      (* extract the necessary info from the place_cond *)
+      iPoseProof (typed_place_cond_incl _ (Uniq κ γ) with "Hincl_k Hcond") as "Hcond'".
+      iDestruct "Hcond'" as "(Hcond' & _)".
+      iDestruct "Hcond'" as "(%Heq & Heq & (#Hub & _))".
+      rewrite (UIP_refl _ _ Heq). cbn.
+      iPoseProof (typed_place_cond_syn_type_eq with "Hcond") as "%Hst_eq".
+      (* close the borrow *)
+      iMod (gvar_update r2 with "Hauth Hrfn") as "(Hauth & Hrfn)".
+      iMod (fupd_mask_subseteq lftE) as "Hcl_F"; first done.
+      iDestruct "Hcred" as "(Hcred1 & Hcred)".
+      iMod ("Hb_cl" with "Hx Hcred1 [Hauth Hl Hb]") as "(Hb & Htok)".
+      { iModIntro. eauto 8 with iFrame. }
+      iMod ("HR" with "Htok") as "$".
+      iMod "Hcl_F" as "_".
+      iModIntro.
+      (* TODO maybe donate the leftover credits *)
+      iSplitL.
+      { rewrite ltype_own_shr_ref_unfold /shr_ltype_own.
+        iExists void*. iFrame. do 3 iR.
+        iPoseProof (pinned_bor_shorten with "Hincl Hb") as "Hb".
+        iModIntro. done. }
+      iDestruct "Hcond" as "(Hcond_ty & Hcond_rfn)".
+      iSplit.
+      + iApply shr_ltype_place_cond_ty; done.
+      + iApply (typed_place_cond_rfn_lift _ _ _ (λ a, #a)). done.
+    - (* shift to OpenedLtype *)
+      iIntros (rt2 lt2 r2) "Hl %Hst' Hb". iModIntro.
+      iDestruct "Hcred" as "(Hcred1 & Hcred)".
+      iApply (opened_ltype_create_uniq_simple with "Hrfn Hauth Hcred1 Hat Hincl HR Hb_cl [] [Hcred']"); first done.
+      { iModIntro. iIntros (?) "Hauth Hc". simp_ltypes.
+        rewrite ltype_own_shr_ref_unfold /shr_ltype_own.
+        iExists _. iFrame. iDestruct "Hc" as ">(% & _ & _ & _ & _ & %r' & -> & >(%l0 & Hl & Hb))".
+        iModIntro. setoid_rewrite ltype_own_core_equiv.
+        iExists _. eauto with iFrame. }
+      { iIntros (?) "Hobs Hat Hcred Hp". simp_ltypes.
+        rewrite ltype_own_shr_ref_unfold /shr_ltype_own.
+        setoid_rewrite ltype_own_core_equiv. rewrite ltype_core_idemp.
+        iModIntro. eauto 8 with iFrame. }
+      { rewrite ltype_own_shr_ref_unfold /shr_ltype_own.
+        iExists void*. do 4 iR.
+        iExists r2. iR. iNext. iModIntro. eauto with iFrame. }
+  Qed.
+
+  Lemma shr_ltype_acc_shared {rt} F π (lt : ltype rt) r l q κ κ' :
+    lftE ⊆ F →
+    rrust_ctx -∗
+    q.[κ] -∗
+    l ◁ₗ[π, Shared κ] #r @ ShrLtype lt κ' -∗
+    ⌜l `has_layout_loc` void*⌝ ∗ loc_in_bounds l 0 (ly_size void*) ∗ |={F}=>
+      ∃ (l' : loc) q', l ↦{q'} l' ∗ (|={F}▷=> l' ◁ₗ[π, Shared κ'] r @ lt) ∗
+    (∀ (lt' : ltype rt) r',
+      l ↦{q'} l' -∗
+      l' ◁ₗ[π, Shared κ'] r' @ lt' -∗ |={F}=>
+      l ◁ₗ[π, Shared κ] #r' @ ShrLtype lt' κ' ∗
+      q.[κ] ∗
+      (∀ bmin,
+      bmin ⊑ₖ Shared κ -∗
+      typed_place_cond bmin lt lt' r r' ={F}=∗
+      typed_place_cond bmin (ShrLtype lt κ') (ShrLtype lt' κ') #r #r')).
+  Proof.
+    iIntros (?) "#(LFT & TIME & LLCTX) Hκ Hb". rewrite {1}ltype_own_shr_ref_unfold /shr_ltype_own.
+    iDestruct "Hb" as "(%ly & %Hst & %Hly & #Hlb & %r' & -> & #Hb)".
+    apply syn_type_has_layout_ptr_inv in Hst. subst ly.
+    iR. iR.
+    iMod (fupd_mask_mono with "Hb") as "(%li & #Hf & #Hl)"; first done.
+    iMod (frac_bor_acc with "LFT Hf Hκ") as "(%q' & >Hpts & Hclf)"; first done.
+    iModIntro. iExists _, _. iFrame.
+    iSplitR. { iApply step_fupd_intro; first done. auto. }
+    iIntros (lt' r'') "Hpts #Hl'".
+    iMod ("Hclf" with "Hpts") as "Htok".
+    iFrame. iSplitL.
+    { iModIntro. rewrite ltype_own_shr_ref_unfold /shr_ltype_own. iExists void*. iFrame "% #".
+      iR. iExists _. iR. iModIntro. iModIntro. iExists _. iFrame "#". }
+    iModIntro. iIntros (bmin) "Hincl Hcond".
+    iDestruct "Hcond" as "(Hcond_ty & Hcond_rfn)".
+    iModIntro. iSplit.
+    + iApply shr_ltype_place_cond_ty; done.
+    + destruct bmin; simpl; done.
+  Qed.
+
+End acc.
+
+
+Section rules.
+  Context `{!typeGS Σ}.
+
+  Global Instance get_lft_names_shr_ref {rt} (ty : type rt) κ lfts lfts' name tree :
+    GetLftNames ty lfts tree lfts' →
+    GetLftNames (shr_ref ty κ) lfts (LftNameTreeRef name tree) (named_lft_update name κ lfts') := λ _, GLN.
+
+  Lemma typed_place_shr_owned {rto} π κ (lt2 : ltype rto) P E L l r wl bmin0 (T : place_cont_t (place_rfn rto)) :
+    (∀ l', typed_place π E L l' lt2 r (Shared κ ⊓ₖ bmin0) (Shared κ) P
+        (λ L' κs l2 b2 bmin rti tyli ri strong weak,
+          T L' (κs) l2 b2 bmin rti tyli ri
+          (option_map (λ strong, mk_strong
+            (λ rti2, (place_rfn (strong.(strong_rt) rti2)))%type
+            (λ rti2 lti2 ri2, ShrLtype (strong.(strong_lt) _ lti2 ri2) κ)
+            (λ rti2 (r : place_rfn rti2), PlaceIn (strong.(strong_rfn) _ r))
+            strong.(strong_R)) strong)
+          (fmap (λ weak,  mk_weak
+            (λ lti2 ri2, ShrLtype (weak.(weak_lt) lti2 ri2) κ)
+            (λ (r : place_rfn rti), PlaceIn (weak.(weak_rfn) r))
+            weak.(weak_R)) weak)))
+    ⊢ typed_place π E L l (ShrLtype lt2 κ) (#r) bmin0 (Owned wl) (DerefPCtx Na1Ord PtrOp true :: P) T.
+  Proof.
+    iIntros "HR" (Φ F ??).
+    iIntros "#(LFT & TIME & LLCTX) #HE HL Hincl0 HP HΦ/=".
+    iPoseProof (shr_ltype_acc_owned F with "[$LFT $TIME $LLCTX] HP") as "(%Hly & Hlb & Hb)"; [done.. | ].
+    iApply fupd_wp. iMod (fupd_mask_subseteq F) as "HclF"; first done.
+    iMod "Hb" as "(%l' & Hl & Hb & Hcl)". iMod "HclF" as "_". iModIntro.
+    iApply (wp_logical_step with "TIME Hcl"); [solve_ndisj.. | ].
+    iApply (wp_deref with "Hl") => //; [solve_ndisj | by apply val_to_of_loc | ].
+    iNext. iIntros (st) "Hl Hcred Hc". iMod (fupd_mask_subseteq F) as "HclF"; first done.
+    iMod "HclF" as "_". iExists l'.
+    iSplitR. { iPureIntro. unfold mem_cast. rewrite val_to_of_loc. done. }
+    iApply ("HR" with "[//] [//] [$LFT $TIME $LLCTX] HE HL [] Hb"). { iApply bor_kind_min_incl_l. }
+    iModIntro. iIntros (L' κs l2 b2 bmin rti tyli ri strong weak) "#Hincl1 Hb Hs".
+    iApply ("HΦ" $! _ _ _ _ bmin _ _ _ _ _ with "Hincl1 Hb").
+    simpl. iSplit.
+    - (* strong *) iDestruct "Hs" as "[Hs _]".
+      destruct strong as [ strong | ]; last done.
+      iIntros (rti2 ltyi2 ri2) "Hl2 Hcond".
+      iMod ("Hs" with "Hl2 Hcond") as "(Hb & Hcond & HR)".
+      iMod ("Hc" $! (Owned false) with "Hl Hb") as "(Hb & _)".
+      iFrame. iPureIntro. simp_ltypes. done.
+    - (* weak *)
+      destruct weak as [ weak | ]; last done.
+      iDestruct "Hs" as "[_ Hs]".
+      iIntros (ltyi2 ri2 bmin').
+      iIntros "Hincl2 Hl2 Hcond".
+      iMod ("Hs" with "Hincl2 Hl2 Hcond") as "(Hb & Hcond & $ & HR)".
+      iMod ("Hc" with "Hl Hb") as "(Hb & Hcond')".
+      iPoseProof ("Hcond'" with "Hcond") as "Hcond".
+      iModIntro. iFrame "HR Hb".
+      iApply typed_place_cond_incl; last iApply "Hcond".
+      + iApply bor_kind_min_incl_r.
+      + iPureIntro. apply place_access_rt_rel_refl.
+  Qed.
+  Global Instance typed_place_shr_owned_inst {rto} E L π κ (lt2 : ltype rto) bmin0 r l wl P :
+    TypedPlace E L π l (ShrLtype lt2 κ) (PlaceIn (r)) bmin0 (Owned wl) (DerefPCtx Na1Ord PtrOp true :: P) | 30 := λ T, i2p (typed_place_shr_owned π κ lt2 P E L l r wl bmin0 T).
+
+  Lemma typed_place_shr_uniq {rto} π κ (lt2 : ltype rto) P E L l r κ' γ bmin0 (T : place_cont_t (place_rfn rto)) :
+    li_tactic (lctx_lft_alive_count_goal E L κ') (λ '(κs, L2),
+    (∀ l', typed_place π E L2 l' lt2 r (Shared κ) (Shared κ) P
+        (λ L3 κs' l2 b2 bmin rti tyli ri strong weak,
+          T L3 (κs' ++ κs) l2 b2 bmin rti tyli ri
+            (* strong branch: fold to OpenedLtype *)
+            (fmap (λ strong, mk_strong (λ rti, (place_rfn (strong.(strong_rt) rti)))
+              (λ rti2 ltyi2 ri2,
+                OpenedLtype (ShrLtype (strong.(strong_lt) _ ltyi2 ri2) κ) (ShrLtype lt2 κ) (ShrLtype lt2 κ) (λ r1 r1', ⌜r1 = r1'⌝) (λ _ _, llft_elt_toks κs))
+              (λ rti2 ri2, #((strong.(strong_rfn) _ ri2)))
+              strong.(strong_R)) strong)
+              (* TODO: maybe we should enable weak accesses *)
+            (* weak branch: just keep the ShrLtype *)
+              (*
+            (fmap (λ weak,  mk_weak
+            (λ lti2 ri2, ShrLtype (weak.(weak_lt) lti2 ri2) κ)
+            (λ (r : place_rfn rti), PlaceIn (weak.(weak_rfn) r))
+            weak.(weak_R)) weak)
+               *)
+              None
+        )))
+    ⊢ typed_place π E L l (ShrLtype lt2 κ) (#r) bmin0 (Uniq κ' γ) (DerefPCtx Na1Ord PtrOp true :: P) T.
+  Proof.
+    rewrite /lctx_lft_alive_count_goal.
+    iIntros "(%κs & %L2 & %Hal & HT)".
+    iIntros (Φ F ??). iIntros "#(LFT & TIME & LLCTX) #HE HL #Hincl0 HP HΦ/=".
+    (* get a token *)
+    iApply fupd_wp. iMod (fupd_mask_subseteq lftE) as "HclF"; first done.
+    iMod (lctx_lft_alive_count_tok lftE with "HE HL") as (q) "(Hκ' & Hclκ' & HL)"; [done.. | ].
+    iMod "HclF" as "_". iMod (fupd_mask_subseteq F) as "HclF"; first done.
+    iPoseProof (shr_ltype_acc_uniq F with "[$LFT $TIME $LLCTX] Hκ' Hclκ' HP") as "(%Hly & Hlb & Hb)"; [done.. | ].
+    iMod "Hb" as "(%l' & Hl & Hb & Hcl)". iMod "HclF" as "_". iModIntro.
+    iApply (wp_logical_step with "TIME Hcl"); [solve_ndisj.. | ].
+    iApply (wp_deref with "Hl") => //; [solve_ndisj | by apply val_to_of_loc | ].
+    iNext. iIntros (st) "Hl Hcred Hc". iMod (fupd_mask_subseteq F) as "HclF"; first done.
+    iMod "HclF" as "_". iExists l'.
+    iSplitR. { iPureIntro. unfold mem_cast. rewrite val_to_of_loc. done. }
+    iApply ("HT" with "[//] [//] [$LFT $TIME $LLCTX] HE HL [] Hb"). { iApply bor_kind_incl_refl. }
+    iModIntro. iIntros (L' κs' l2 b2 bmin rti tyli ri strong weak) "#Hincl1 Hb Hs".
+    iApply ("HΦ" $! _ _ _ _ bmin _ _ _ _ _ with "Hincl1 Hb").
+    simpl. iSplit.
+    - (* strong *) iDestruct "Hs" as "[Hs _]".
+      destruct strong as [ strong | ]; last done.
+      iIntros (rti2 ltyi2 ri2) "Hl2 Hcond".
+      iMod ("Hs" with "Hl2 Hcond") as "(Hb & %Hcond & HR)".
+      iDestruct "Hc" as "[_ Hc]". simpl.
+      iMod ("Hc" with "Hl [] Hb") as "Hb".
+      { rewrite Hcond. done. }
+      iFrame. iPureIntro. simp_ltypes. done.
+    - (* weak *)
+      destruct weak as [ weak | ]; last done.
+      iDestruct "Hs" as "[_ Hs]".
+      done.
+      (*
+      iIntros (ltyi2 ri2 bmin').
+      iIntros "Hincl2 Hl2 Hcond".
+      iDestruct "Hc" as "[Hc _]". simpl.
+      iMod ("Hs" with "Hincl2 Hl2 Hcond") as "(Hb & Hcond & Htoks & HR)".
+
+      iMod ("Hc" with "Hl Hb []") as "(Hb & Hcond')".
+      iPoseProof ("Hcond'" with "Hcond") as "Hcond".
+      iModIntro. iFrame "HR Hb".
+      iApply typed_place_cond_incl; last iApply "Hcond".
+      + iApply bor_kind_min_incl_r.
+      + iPureIntro. apply place_access_rt_rel_refl.
+       *)
+  Qed.
+  Global Instance typed_place_shr_uniq_inst {rto} E L π κ (lt2 : ltype rto) bmin0 r l κ' γ P :
+    TypedPlace E L π l (ShrLtype lt2 κ) (#r) bmin0 (Uniq κ' γ) (DerefPCtx Na1Ord PtrOp true :: P) | 30 := λ T, i2p (typed_place_shr_uniq π κ lt2 P E L l r κ' γ bmin0 T).
+
+  Lemma typed_place_shr_shared {rto} π E L (lt2 : ltype rto) P l r κ κ' bmin0 (T : place_cont_t (place_rfn rto)) :
+    li_tactic (lctx_lft_alive_count_goal E L κ') (λ '(κs, L'),
+      (∀ l', typed_place π E L' l' lt2 r (Shared κ ⊓ₖ bmin0) (Shared κ) P
+        (λ L'' κs' l2 b2 bmin rti tyli ri strong weak,
+          T L'' (κs ++ κs') l2 b2 (Shared κ' ⊓ₖ bmin) rti tyli ri
+            (* strong branch: fold to ShadowedLtype *)
+              None (* TODO *)
+            (*(fmap (λ strong, mk_strong (λ rti, (place_rfn (strong.(strong_rt) rti) * gname)%type)*)
+              (*(λ rti2 ltyi2 ri2,*)
+                (*OpenedLtype (MutLtype (strong.(strong_lt) _ ltyi2 ri2) κ) (MutLtype lt2 κ) (MutLtype lt2 κ) (λ r1 r1', ⌜r1 = r1'⌝) (λ _ _, llft_elt_toks κs))*)
+              (*(λ rti2 ri2, #((strong.(strong_rfn) _ ri2), γ))*)
+              (*strong.(strong_R)) strong)*)
+            (* weak branch: just keep the MutLtype *)
+            (fmap (λ weak, mk_weak (λ lti' ri', ShrLtype (weak.(weak_lt) lti' ri') κ) (λ (r : place_rfn rti), #(weak.(weak_rfn) r)) weak.(weak_R)) weak))))
+    ⊢ typed_place π E L l (ShrLtype lt2 κ) #r bmin0 (Shared κ') (DerefPCtx Na1Ord PtrOp true :: P) T.
+  Proof.
+    rewrite /lctx_lft_alive_count_goal.
+    iIntros "(%κs & %L2 & %Hal & HT)".
+    iIntros (Φ F ??). iIntros "#(LFT & TIME & LLCTX) #HE HL #Hincl0 HP HΦ/=".
+    (* get a token *)
+    iApply fupd_wp. iMod (fupd_mask_subseteq lftE) as "HclF"; first done.
+    iMod (lctx_lft_alive_count_tok lftE with "HE HL") as (q) "(Hκ' & Hclκ' & HL)"; [done.. | ].
+    iMod "HclF" as "_". iMod (fupd_mask_subseteq F) as "HclF"; first done.
+    iPoseProof (shr_ltype_acc_shared F with "[$LFT $TIME $LLCTX] Hκ' HP") as "(%Hly & Hlb & Hb)"; [done.. | ].
+    iMod "Hb" as "(%l' & %q' & Hl & >Hb & Hcl)". iMod "HclF" as "_".
+    iModIntro. iApply wp_fupd. iApply (wp_deref with "Hl") => //; [solve_ndisj | by apply val_to_of_loc | ].
+    iNext.
+    iIntros (st) "Hl Hcred". iMod (fupd_mask_mono with "Hb") as "#Hb"; first done.
+    iExists l'.
+    iSplitR. { iPureIntro. unfold mem_cast. rewrite val_to_of_loc. done. }
+    iApply ("HT" with "[//] [//] [$LFT $TIME $LLCTX] HE HL [] Hb"). { iApply bor_kind_min_incl_l. }
+    iModIntro. iIntros (L'' κs' l2 b2 bmin rti tyli ri strong weak) "#Hincl1 Hb' Hs".
+    iApply ("HΦ" $! _ _ _ _ (Shared κ' ⊓ₖ bmin) _ _ _ _ _ with "[Hincl1] Hb'").
+    { iApply bor_kind_incl_trans; last iApply "Hincl1". iApply bor_kind_min_incl_r. }
+    simpl. iSplit.
+    - (* strong update *)
+      done.
+    - (* weak update *)
+      destruct weak as [ weak | ]; last done.
+      iDestruct "Hs" as "(_ & Hs)".
+      iIntros (ltyi2 ri2 bmin') "#Hincl2 Hl2 Hcond".
+      iMod ("Hs" with "[Hincl2] Hl2 Hcond") as "(Hb' & Hcond & ? & HR)".
+      { iApply bor_kind_incl_trans; first iApply "Hincl2". iApply bor_kind_min_incl_r. }
+      simpl.
+      iMod ("Hcl" with "Hl Hb'") as "(Hb' & Hκ' & Hcond')".
+      iFrame. rewrite llft_elt_toks_app.
+      iMod (fupd_mask_mono with "(Hclκ' Hκ')") as "?"; first done.
+      iFrame. iApply "Hcond'".
+      + done.
+      + iApply typed_place_cond_incl; last done.
+        iApply bor_kind_min_incl_r.
+  Qed.
+  Global Instance typed_place_shr_shared_inst {rto} E L π κ κ' (lt2 : ltype rto) bmin0 r l P :
+    TypedPlace E L π l (ShrLtype lt2 κ) (#r) bmin0 (Shared κ') (DerefPCtx Na1Ord PtrOp true :: P) | 30 := λ T, i2p (typed_place_shr_shared π E L lt2 P l r κ κ' bmin0 T).
+
+  (* TODO more place instances *)
+
+  Lemma typed_place_ofty_shr {rt} `{Inhabited rt} π E L l (ty : type rt) κ (r : place_rfn (place_rfn rt)) bmin0 b P T :
+    typed_place π E L l (ShrLtype (◁ ty) κ) r bmin0 b P T
+    ⊢ typed_place π E L l (◁ (shr_ref ty κ)) r bmin0 b P T.
+  Proof.
+    iIntros "Hp". iApply typed_place_eqltype; last done.
+    iIntros (?) "HL CTX HE".
+    iIntros (??). iApply ltype_eq_sym. iApply shr_ref_unfold.
+  Qed.
+  Global Instance typed_place_ofty_shr_inst {rt} `{Inhabited rt} π E L l (ty : type rt) κ (r : place_rfn (place_rfn rt)) bmin0 b P :
+    TypedPlace E L π l (◁ (shr_ref ty κ))%I r bmin0 b P | 30 := λ T, i2p (typed_place_ofty_shr π E L l ty κ r bmin0 b P T).
+
+  Lemma stratify_ltype_shr_owned {rt} π E L mu mdu ma {M} (ml : M) l (lt : ltype rt) κ (r : (place_rfn rt)) wl
+      (T : stratify_ltype_cont_t) :
+    (∀ l', stratify_ltype π E L mu mdu ma ml l' lt r (Shared κ) (λ L' R rt' lt' r',
+      match ma with
+      | StratRefoldFull =>
+          ∃ (_ : Inhabited rt'), cast_ltype_to_type E L' lt' (λ ty', T L' R _ (◁ (shr_ref ty' κ))%I (#r'))
+      | _ => T L' R _ (ShrLtype lt' κ) (#r')
+      end))
+    ⊢ stratify_ltype π E L mu mdu ma ml l (ShrLtype lt κ) (#r) (Owned wl) T.
+  Proof.
+    iIntros "Hs". iIntros (?? ?) "#(LFT & TIME & LLCTX) #HE HL Hb".
+    iPoseProof (shr_ltype_acc_owned F with "[$LFT $TIME $LLCTX] Hb") as "Hb"; [done.. | ].
+    iDestruct "Hb" as "(%Hly & #Hlb & >(%l' & Hl & Hb & Hcl))".
+    iPoseProof ("Hs" with "[//] [//] [$LFT $TIME $LLCTX] HE HL Hb") as "Hb".
+    iMod "Hb" as "(%L' & %R & %rt' & %lt' & %r' & HL & %Hcond & Hstep & Hc)".
+    destruct (decide (ma = StratRefoldFull)) as [Heq | ].
+    - subst ma.
+      iDestruct "Hc" as "(% & %ty' & %Heq & HT)".
+      iPoseProof (eqltype_use F with "[$LFT $TIME $LLCTX] HE HL") as "(Hvs & HL)"; [done | .. ].
+      { apply full_eqltype_alt. apply Heq. }
+      (*iPoseProof (eqltype_acc with "[$LFT $TIME $LLCTX] HE HL") as "#Heq"; first done.*)
+      iModIntro. iExists L', R, _, _, _. iFrame.
+      iSplitR. { simp_ltypes. done. }
+      iApply logical_step_fupd.
+      iApply (logical_step_compose with "Hcl").
+      iApply (logical_step_compose with "Hstep").
+      iApply logical_step_intro. iIntros "(Hb & $) Hcl".
+      iMod ("Hvs" with "Hb") as "Hb".
+      iMod ("Hcl" $! (Shared κ) with "Hl Hb") as "(Hb & _)".
+      iDestruct (shr_ref_unfold_1 ty' κ (Owned wl)) as "(_ & #Hi & _)".
+      iMod (fupd_mask_mono with "(Hi Hb)") as "$"; first done.
+      done.
+    - iAssert (T L' R _ (ShrLtype lt' κ) (#r')) with "[Hc]" as "Hc".
+      { destruct ma; done. }
+      iModIntro. iExists L', R, _, _, _. iFrame.
+      iSplitR. { simp_ltypes; done. }
+      iApply logical_step_fupd.
+      iApply (logical_step_compose with "Hcl").
+      iApply (logical_step_compose with "Hstep").
+      iApply logical_step_intro. iIntros "(Hb & $) Hcl".
+      by iMod ("Hcl" $! (Shared κ) with "Hl Hb") as "($ & _)".
+  Qed.
+  Global Instance stratify_ltype_shr_owned_none_inst {rt} π E L mdu ma {M} (ml : M) l (lt : ltype rt) κ (r : (place_rfn rt)) wl :
+    StratifyLtype π E L StratMutNone mdu ma ml l (ShrLtype lt κ) (#r) (Owned wl) := λ T, i2p (stratify_ltype_shr_owned π E L StratMutNone mdu ma ml l lt κ r wl T).
+
+  (* TODO Uniq *)
+
+  (* Notes on stratification of [Shared]:
+     basically:
+     when we are accessing, we are unfolding
+
+    - in principle, this should "just work" by operating under these laters.
+      Below shared references, the amount of unfolding we could have done is very limited: basically, we can only have
+        ShrBlocked or Shadowed.
+      For Shadowed: should easily be able to take it back.
+      For ShrBlocked: this might be more of a problem.
+          We actually need to execute the viewshift for the inheritance, right.
+          However, do we ever have nested shrblocked (ie below Shared) in practice?
+          => No. I cannot initialize a shrblocked from that, because I cannot initialize sharing.
+            Rather, creating a shr reference from a shared place should copy the existing sharing.
+
+      Then: I basically just want to be able to execute this stratification below the later.
+        Issue with using this stratify: the lifetime context stuff.
+        But in principle, shared stratification should also not use the lifetime context stuff.
+
+      Maybe have a separate notion of shared stratification to account for that?
+      That basically should just take the thing unter an iterated step_fupdN and also only need to provide the stratified thing under a step_fupdN.
+
+      Eventually: what happens if we do interior mutability?
+        then we will actually open an invariant and get some tokens for stuff back.
+        Though we might just want to have that for primitive ofty things, not nested
+
+      In the shared case, can we just set this up differently altogether?
+        Maybe just require subtyping of core?
+        Can Shared stuff always go directly to the core?
+        => Yes, I think so, for now.
+        Alternative: directly go to the core.
+          i.e. would have to prove that for Shared we can always go to the core.
+          For more advanced sharing patterns where we actually want to have shrblocked, this might not work though. but that is anyways far in the future now.
+          This is anyways slightly incompatible with the current model/needs work.
+
+      Options now:
+      - have stratify_ltype version for Shared that operates below the laters. Basically, this would just be a fancy version of subtyping though.
+      - use subtyping, by proving that it is a subtype of the core, and then folding that.
+      - use the core, but have proved it once and for all.
+
+    - maybe we also want to have the depth certificates here? *)
+  (* This is loosing information by dropping potential [ShadowedLtype], so we should only do it when really necessary. *)
+  Lemma stratify_ltype_shared {rt} π E L mu mdu ma {M} (ml : M) l (lt : ltype rt) κ (r : place_rfn rt) (T : stratify_ltype_cont_t):
+    (cast_ltype_to_type E L (ltype_core lt) (λ ty', T L True _ (◁ ty')%I (r)))
+    ⊢ stratify_ltype π E L mu mdu ma ml l lt r (Shared κ) T.
+  Proof.
+    iIntros "HT". iIntros (???) "#CTX #HE HL Hl".
+    iDestruct "HT" as "(%ty & %Heq & HT)".
+    iPoseProof (full_eqltype_acc with "CTX HE HL") as "#Heq"; first apply Heq.
+    iPoseProof (ltype_own_shared_to_core with "Hl") as "Hl".
+    iDestruct ("Heq" $! (Shared κ) r) as "((%Hsteq & #Hinc & _) & _)".
+    iPoseProof ("Hinc" with "Hl") as "Hl".
+    iExists L, _, _, _, _. iFrame.
+    iModIntro. iSplitR. { simp_ltypes. done. }
+    iApply logical_step_intro. iSplitL; done.
+  Qed.
+  Global Instance stratify_ltype_shared_inst1 {rt} π E L mu mdu {M} (ml : M) l (lt : ltype rt) κ (r : place_rfn rt) :
+    StratifyLtype π E L mu mdu StratRefoldFull ml l lt r (Shared κ) :=
+    λ T, i2p (stratify_ltype_shared π E L mu mdu StratRefoldFull ml l lt κ r T).
+  Global Instance stratify_ltype_shared_inst2 {rt} π E L mu mdu {M} (ml : M) l (lt : ltype rt) κ (r : place_rfn rt) :
+    StratifyLtype π E L mu mdu StratRefoldOpened ml l lt r (Shared κ) :=
+    λ T, i2p (stratify_ltype_shared π E L mu mdu StratRefoldOpened ml l lt κ r T).
+
+  Lemma stratify_ltype_ofty_shr {rt} `{Inhabited rt} π E L mu ma {M} (ml : M) l (ty : type rt) κ (r : place_rfn (place_rfn rt)) b T :
+    stratify_ltype π E L mu StratDoUnfold ma ml l (ShrLtype (◁ ty) κ) r b T
+    ⊢ stratify_ltype π E L mu StratDoUnfold ma ml l (◁ (shr_ref ty κ)) r b T.
+  Proof.
+    iIntros "Hp". iApply stratify_ltype_eqltype; iFrame.
+    iPureIntro. iIntros (?) "HL CTX HE".
+    iApply ltype_eq_sym. iApply shr_ref_unfold.
+  Qed.
+  Global Instance stratify_ltype_ofty_shr_inst {rt} `{Inhabited rt} π E L mu ma {M} (ml : M) l (ty : type rt) κ (r : place_rfn (place_rfn rt)) b :
+    StratifyLtype π E L mu StratDoUnfold ma ml l (◁ (shr_ref ty κ))%I r b | 30 := λ T, i2p (stratify_ltype_ofty_shr π E L mu ma ml l ty κ r b T).
+  (** prove_place_cond instances *)
+  (* These need to have a lower priority than the ofty_refl instance (level 2) and the unblocking instances (level 5), but higher than the trivial "no" instance *)
+  Lemma prove_place_cond_unfold_shr_l E L {rt1 rt2} `{Inhabited rt1} (ty : type rt1) (lt : ltype rt2) κ k T :
+    prove_place_cond E L k (ShrLtype (◁ ty) κ) lt T
+    ⊢ prove_place_cond E L k (◁ (shr_ref ty κ)) lt T.
+  Proof.
+    iApply prove_place_cond_eqltype_l. apply symmetry. apply shr_ref_unfold_full_eqltype; done.
+  Qed.
+  Global Instance prove_place_cond_unfold_shr_l_inst E L {rt1 rt2} `{Inhabited rt1} (ty : type rt1) (lt : ltype rt2) κ k :
+    ProvePlaceCond E L k (◁ (shr_ref ty κ))%I lt | 10 := λ T, i2p (prove_place_cond_unfold_shr_l E L ty lt κ k T).
+  Lemma prove_place_cond_unfold_shr_r E L {rt1 rt2} `{Inhabited rt1} (ty : type rt1) (lt : ltype rt2) κ k T :
+    prove_place_cond E L k lt (ShrLtype (◁ ty) κ) T
+    ⊢ prove_place_cond E L k lt (◁ (shr_ref ty κ)) T.
+  Proof.
+    iApply prove_place_cond_eqltype_r. apply symmetry. apply shr_ref_unfold_full_eqltype; done.
+  Qed.
+  Global Instance prove_place_cond_unfold_shr_r_inst E L {rt1 rt2} `{Inhabited rt1} (ty : type rt1) (lt : ltype rt2) κ k :
+    ProvePlaceCond E L k lt (◁ (shr_ref ty κ))%I | 10 := λ T, i2p (prove_place_cond_unfold_shr_r E L ty lt κ k T).
+
+  Lemma prove_place_cond_ShrLtype E L {rt1 rt2} (lt1 : ltype rt1) (lt2 : ltype rt2) κ k T :
+    prove_place_cond E L (Shared κ ⊓ₖ k) lt1 lt2 (λ upd, T $ access_result_lift place_rfn upd)
+    ⊢ prove_place_cond E L k (ShrLtype lt1 κ) (ShrLtype lt2 κ) T.
+  Proof.
+    (* TODO *)
+  Abort.
+
+  (** Typing rule for shared borrowing, manually applied by the tactics *)
+  Lemma type_shr_bor E L T e π κ_name ty_annot :
+    (∃ M, named_lfts M ∗ li_tactic (compute_map_lookup_nofail_goal M κ_name) (λ κ,
+    (named_lfts M -∗ typed_borrow_shr π E L e κ ty_annot (λ L' v rt ty r, T L' v (place_rfn rt) (shr_ref ty κ) (r)))))
+    ⊢ typed_val_expr π E L (&ref{Shr, ty_annot, κ_name} e)%E T.
+  Proof.
+    rewrite /compute_map_lookup_nofail_goal.
+    iIntros "(%M & Hnamed & %κ & _ & HT)". iIntros (Φ) "#(LFT & TIME & LLCTX) #HE HL Hna HΦ".
+    wp_bind. iSpecialize ("HT" with "Hnamed"). iApply ("HT" $! _ ⊤ with "[//] [//] [//] [$LFT $TIME $LLCTX] HE HL Hna").
+    iIntros (l) "HT".
+    unfold Ref. wp_bind. iApply ewp_fupd.
+    iApply (wp_logical_step with "TIME HT"); [solve_ndisj.. | ].
+    iApply wp_skip. iNext. iIntros "Hcred HT !> !>".
+    iApply (wp_logical_step with "TIME HT"); [solve_ndisj.. | ].
+    iApply wp_skip. iNext. iIntros "Hcred' HT".
+    iMod ("HT" with "Hcred'") as (L' rt ty r r' ly) "(#Hrfn & #Hshr & %Halg & %Hly & #Hlb & #Hsc & HL & Hna & HT)".
+    iModIntro. iApply ("HΦ" with "HL Hna [Hshr] HT").
+    iExists l, ly, r'. iSplitR; first done. iFrame "Hlb Hrfn Hsc %".
+    iModIntro. iModIntro. done.
+  Qed.
+
+  (** cast_ltype *)
+  Lemma cast_ltype_to_type_shr E L {rt} `{Inhabited rt} (lt : ltype rt) κ T  :
+    cast_ltype_to_type E L lt (λ ty, T (shr_ref ty κ))
+    ⊢ cast_ltype_to_type E L (ShrLtype lt κ) T.
+  Proof.
+    iIntros "Hs". iDestruct "Hs" as "(%ty & %Heq & HT)".
+    iExists (shr_ref ty κ). iFrame "HT". iPureIntro.
+    by apply shr_ref_unfold_full_eqltype.
+  Qed.
+  Global Instance cast_ltype_to_type_shr_inst E L {rt} `{Inhabited rt} (lt : ltype rt) κ :
+    CastLtypeToType E L (ShrLtype lt κ) :=
+    λ T, i2p (cast_ltype_to_type_shr E L lt κ T).
+
+  (** subtyping *)
+  Lemma weak_subtype_shr_in E L {rt1 rt2} (ty1 : type rt1) (ty2 : type rt2) κ1 κ2 r1 r2 T :
+    (⌜lctx_lft_incl E L κ2 κ1⌝ ∗ weak_subtype E L r1 r2 ty1 ty2 T)
+    ⊢ weak_subtype E L #r1 #r2 (shr_ref ty1 κ1) (shr_ref ty2 κ2) T.
+  Proof.
+    iIntros "(%Hincl & HT)". iIntros (??) "#CTX #HE HL".
+    iPoseProof (lctx_lft_incl_incl with "HL") as "#Hincl"; first done.
+    iSpecialize ("Hincl" with "HE").
+    iMod ("HT" with "[//] CTX HE HL") as "(#Hsub & $ & $)".
+    iApply shr_ref_type_incl_in; done.
+  Qed.
+  Global Instance weak_subtype_shr_in_inst E L {rt1 rt2} (ty1 : type rt1) (ty2 : type rt2) κ1 κ2 r1 r2 :
+    Subtype E L #r1 #r2 (shr_ref ty1 κ1) (shr_ref ty2 κ2) | 10:= λ T, i2p (weak_subtype_shr_in E L ty1 ty2 κ1 κ2 r1 r2 T).
+
+  Lemma weak_subtype_shr E L {rt} `{!Inhabited rt} (ty1 ty2 : type rt) κ1 κ2 r1 r2 T :
+    (⌜r1 = r2⌝ ∗ ⌜lctx_lft_incl E L κ2 κ1⌝ ∗ mut_subtype E L ty1 ty2 T)
+    ⊢ weak_subtype E L r1 r2 (shr_ref ty1 κ1) (shr_ref ty2 κ2) T.
+  Proof.
+    iIntros "(-> & %Hincl & %Hsubt & HT)". iIntros (??) "#CTX #HE HL".
+    iPoseProof (lctx_lft_incl_incl with "HL") as "#Hincl"; first done.
+    iSpecialize ("Hincl" with "HE").
+    iPoseProof (full_subtype_acc with "HE HL") as "#Hsub"; first done.
+    iFrame. unshelve iApply shr_ref_type_incl; done.
+  Qed.
+  Global Instance weak_subtype_shr_inst E L {rt} `{!Inhabited rt} (ty1 ty2 : type rt) κ1 κ2 r1 r2 :
+    Subtype E L r1 r2 (shr_ref ty1 κ1) (shr_ref ty2 κ2) | 11 := λ T, i2p (weak_subtype_shr E L ty1 ty2 κ1 κ2 r1 r2 T).
+
+  Lemma weak_subtype_shr_evar_lft E L {rt} (ty1 ty2 : type rt) κ1 κ2 r1 r2 T `{!IsProtected κ2} :
+    ⌜κ1 = κ2⌝ ∗ weak_subtype E L r1 r2 (shr_ref ty1 κ1) (shr_ref ty2 κ1) T
+    ⊢ weak_subtype E L r1 r2 (shr_ref ty1 κ1) (shr_ref ty2 κ2) T.
+  Proof. iIntros "(<- & $)". Qed.
+  Global Instance weak_subtype_shr_evar_lft_inst E L {rt} (ty1 ty2 : type rt) κ1 κ2 r1 r2 `{!IsProtected κ2} :
+    Subtype E L r1 r2 (shr_ref ty1 κ1) (shr_ref ty2 κ2) | 9 := λ T, i2p (weak_subtype_shr_evar_lft E L ty1 ty2 κ1 κ2 r1 r2 T).
+
+  Lemma mut_subtype_shr E L {rt} `{!Inhabited rt} (ty1 ty2 : type rt) κ1 κ2 T :
+    ⌜lctx_lft_incl E L κ2 κ1⌝ ∗ mut_subtype E L ty1 ty2 T
+    ⊢ mut_subtype E L (shr_ref ty1 κ1) (shr_ref ty2 κ2) T.
+  Proof.
+    iIntros "(%Hincl & %Hsub & $)". iPureIntro. by eapply shr_ref_full_subtype.
+  Qed.
+  Global Instance mut_subtype_shr_inst E L {rt} `{!Inhabited rt} (ty1 ty2 : type rt) κ1 κ2 :
+    MutSubtype E L (shr_ref ty1 κ1) (shr_ref ty2 κ2) | 10 := λ T, i2p (mut_subtype_shr E L ty1 ty2 κ1 κ2 T).
+  Lemma mut_subtype_shr_evar_lft E L {rt} (ty1 ty2 : type rt) κ1 κ2 T `{!IsProtected κ2} :
+    ⌜κ1 = κ2⌝ ∗ mut_subtype E L (shr_ref ty1 κ1) (shr_ref ty2 κ1) T
+    ⊢ mut_subtype E L (shr_ref ty1 κ1) (shr_ref ty2 κ2) T.
+  Proof. iIntros "(<- & $)". Qed.
+  Global Instance mut_subtype_shr_evar_lft_inst E L {rt} (ty1 ty2 : type rt) κ1 κ2 `{!IsProtected κ2} :
+    MutSubtype E L (shr_ref ty1 κ1) (shr_ref ty2 κ2) | 9:= λ T, i2p (mut_subtype_shr_evar_lft E L ty1 ty2 κ1 κ2 T).
+
+  Lemma mut_eqtype_shr E L {rt} `{!Inhabited rt} (ty1 ty2 : type rt) κ1 κ2 T :
+    ⌜lctx_lft_incl E L κ2 κ1⌝ ∗ ⌜lctx_lft_incl E L κ1 κ2⌝ ∗ mut_eqtype E L ty1 ty2 T
+    ⊢ mut_eqtype E L (shr_ref ty1 κ1) (shr_ref ty2 κ2) T.
+  Proof.
+    iIntros "(%Hincl & %Hsub & %Hsub2 & $)". iPureIntro. split.
+    - eapply shr_ref_full_subtype; first done. by eapply full_eqtype_subtype_l.
+    - eapply shr_ref_full_subtype; first done. by eapply full_eqtype_subtype_r.
+  Qed.
+  Global Instance mut_eqtype_shr_inst E L {rt} `{!Inhabited rt} (ty1 ty2 : type rt) κ1 κ2 :
+    MutEqtype E L (shr_ref ty1 κ1) (shr_ref ty2 κ2) | 10 := λ T, i2p (mut_eqtype_shr E L ty1 ty2 κ1 κ2 T).
+  Lemma mut_eqtype_shr_evar_lft E L {rt} (ty1 ty2 : type rt) κ1 κ2 T `{!IsProtected κ2} :
+    ⌜κ1 = κ2⌝ ∗ mut_eqtype E L (shr_ref ty1 κ1) (shr_ref ty2 κ1) T
+    ⊢ mut_eqtype E L (shr_ref ty1 κ1) (shr_ref ty2 κ2) T.
+  Proof. iIntros "(<- & $)". Qed.
+  Global Instance mut_eqtype_shr_evar_lft_inst E L {rt} (ty1 ty2 : type rt) κ1 κ2 `{!IsProtected κ2} :
+    MutEqtype E L (shr_ref ty1 κ1) (shr_ref ty2 κ2) | 9:= λ T, i2p (mut_eqtype_shr_evar_lft E L ty1 ty2 κ1 κ2 T).
+
+  (** subltyping *)
+  Lemma weak_subltype_shr_owned_in E L {rt1 rt2} (lt1 : ltype rt1) (lt2 : ltype rt2) wl κ1 κ2 r1 r2 T :
+    (∃ r2', ⌜r2 = #r2'⌝ ∗ ⌜lctx_lft_incl E L κ2 κ1⌝ ∗ weak_subltype E L (Shared κ1) r1 r2' lt1 lt2 T)
+    ⊢ weak_subltype E L (Owned wl) #r1 r2 (ShrLtype lt1 κ1) (ShrLtype lt2 κ2) T.
+  Proof.
+    iIntros "(%r2' & -> & %Hincl & HT)" (??) "#CTX #HE HL".
+    iMod ("HT" with "[//] CTX HE HL") as "(Hincl' & HL & $)".
+    iPoseProof (lctx_lft_incl_incl with "HL") as "#Hincl"; first done.
+    iSpecialize ("Hincl" with "HE"). iFrame.
+    iApply (shr_ltype_incl_owned_in with "Hincl'").
+    done.
+  Qed.
+  Global Instance weak_subltype_shr_owned_in_inst E L {rt1 rt2} (lt1 : ltype rt1) (lt2 : ltype rt2) wl κ1 κ2 r1 r2 :
+    SubLtype E L (Owned wl) #r1 r2 (ShrLtype lt1 κ1) (ShrLtype lt2 κ2) | 10 := λ T, i2p (weak_subltype_shr_owned_in E L lt1 lt2 wl κ1 κ2 r1 r2 T).
+
+ Lemma weak_subltype_shr_owned E L {rt} (lt1 : ltype rt) (lt2 : ltype rt) wl κ1 κ2 r1 r2 T :
+    (⌜r1 = r2⌝ ∗ ⌜lctx_lft_incl E L κ2 κ1⌝ ∗ mut_subltype E L lt1 lt2 T)
+    ⊢ weak_subltype E L (Owned wl) r1 r2 (ShrLtype lt1 κ1) (ShrLtype lt2 κ2) T.
+  Proof.
+    iIntros "(-> & %Hincl & %Hsubt & HT)" (??) "#CTX #HE HL".
+    iPoseProof (full_subltype_acc with "CTX HE HL") as "#Hsub"; first apply Hsubt.
+    iPoseProof (lctx_lft_incl_incl with "HL") as "#Hincl"; first done.
+    iSpecialize ("Hincl" with "HE"). iFrame.
+    iApply (shr_ltype_incl_owned); last done.
+    iApply "Hsub".
+  Qed.
+  Global Instance weak_subltype_shr_owned_inst E L {rt} (lt1 : ltype rt) (lt2 : ltype rt) wl κ1 κ2 r1 r2 :
+    SubLtype E L (Owned wl) r1 r2 (ShrLtype lt1 κ1) (ShrLtype lt2 κ2) | 11 := λ T, i2p (weak_subltype_shr_owned E L lt1 lt2 wl κ1 κ2 r1 r2 T).
+
+  Lemma weak_subltype_shr_shared_in E L {rt1 rt2} (lt1 : ltype rt1) (lt2 : ltype rt2) κ κ1 κ2 r1 r2 T :
+    (∃ r2', ⌜r2 = #r2'⌝ ∗ ⌜lctx_lft_incl E L κ2 κ1⌝ ∗ weak_subltype E L (Shared (κ1)) r1 r2' lt1 lt2 T)
+    ⊢ weak_subltype E L (Shared κ) #r1 r2 (ShrLtype lt1 κ1) (ShrLtype lt2 κ2) T.
+  Proof.
+    iIntros "(%r2' & -> & %Hincl & HT)" (??) "#CTX #HE HL".
+    iMod ("HT" with "[//] CTX HE HL") as "(Hincl' & HL & $)".
+    iPoseProof (lctx_lft_incl_incl with "HL") as "#Hincl"; first done.
+    iSpecialize ("Hincl" with "HE"). iFrame.
+    iApply (shr_ltype_incl_shared_in with "[Hincl']"); last done.
+    done.
+  Qed.
+  Global Instance weak_subltype_shr_shared_in_inst E L {rt1 rt2} (lt1 : ltype rt1) (lt2 : ltype rt2) κ κ1 κ2 r1 r2 :
+    SubLtype E L (Shared κ) #r1 r2 (ShrLtype lt1 κ1) (ShrLtype lt2 κ2) | 10 := λ T, i2p (weak_subltype_shr_shared_in E L lt1 lt2 κ κ1 κ2 r1 r2 T).
+
+  Lemma weak_subltype_shr_shared E L {rt} (lt1 : ltype rt) (lt2 : ltype rt) κ κ1 κ2 r1 r2 T :
+    (⌜r1 = r2⌝ ∗ ⌜lctx_lft_incl E L κ2 κ1⌝ ∗ mut_subltype E L lt1 lt2 T)
+    ⊢ weak_subltype E L (Shared κ) r1 r2 (ShrLtype lt1 κ1) (ShrLtype lt2 κ2) T.
+  Proof.
+    iIntros "(-> & %Hincl & %Hsubt & HT)" (??) "#CTX #HE HL".
+    iPoseProof (full_subltype_acc with "CTX HE HL") as "#Hsub"; first apply Hsubt.
+    iPoseProof (lctx_lft_incl_incl with "HL") as "#Hincl"; first done.
+    iSpecialize ("Hincl" with "HE"). iFrame.
+    iApply (shr_ltype_incl_shared); last done.
+    iApply "Hsub".
+  Qed.
+  Global Instance weak_subltype_shr_shared_inst E L {rt} (lt1 : ltype rt) (lt2 : ltype rt) κ κ1 κ2 r1 r2 :
+    SubLtype E L (Shared κ) r1 r2 (ShrLtype lt1 κ1) (ShrLtype lt2 κ2) | 11 := λ T, i2p (weak_subltype_shr_shared E L lt1 lt2 κ κ1 κ2 r1 r2 T).
+
+  (* Base instance that will trigger, e.g., for Uniq or PlaceGhost refinements *)
+  Lemma weak_subltype_shr_base E L {rt} (lt1 lt2 : ltype rt) k κ1 κ2 r1 r2 T :
+    ⌜r1 = r2⌝ ∗ ⌜lctx_lft_incl E L κ2 κ1⌝ ∗ ⌜lctx_lft_incl E L κ1 κ2⌝ ∗ mut_eqltype E L lt1 lt2 T
+    ⊢ weak_subltype E L k r1 r2 (ShrLtype lt1 κ1) (ShrLtype lt2 κ2) T.
+  Proof.
+    iIntros "(<- & %Hincl1 & %Hincl2 & %Hsubt & T)" (??) "#CTX #HE HL".
+    iPoseProof (full_eqltype_acc with "CTX HE HL") as "#Hincl"; first done.
+    iPoseProof (lctx_lft_incl_incl with "HL") as "#Hincl1"; first apply Hincl1.
+    iSpecialize ("Hincl1" with "HE").
+    iPoseProof (lctx_lft_incl_incl with "HL") as "#Hincl2"; first apply Hincl2.
+    iSpecialize ("Hincl2" with "HE").
+    iFrame. iApply shr_ltype_incl; done.
+  Qed.
+  Global Instance weak_subltype_shr_base_inst E L {rt} (lt1 lt2 : ltype rt) k κ1 κ2 r1 r2 :
+    SubLtype E L k r1 r2 (ShrLtype lt1 κ1) (ShrLtype lt2 κ2) | 20 := λ T, i2p (weak_subltype_shr_base E L lt1 lt2 k κ1 κ2 r1 r2 T).
+
+  Lemma weak_subltype_shr_evar_lft E L {rt} (lt1 lt2 : ltype rt) k κ1 κ2 r1 r2 T `{!IsProtected κ2} :
+    ⌜κ1 = κ2⌝ ∗ weak_subltype E L k r1 r2 (ShrLtype lt1 κ1) (ShrLtype lt2 κ1) T
+    ⊢ weak_subltype E L k r1 r2 (ShrLtype lt1 κ1) (ShrLtype lt2 κ2) T.
+  Proof. iIntros "(<- & $)". Qed.
+  Global Instance weak_subltype_shr_evar_lft_inst E L {rt} (lt1 lt2 : ltype rt) k κ1 κ2 r1 r2 `{!IsProtected κ2} :
+    SubLtype E L k r1 r2 (ShrLtype lt1 κ1) (ShrLtype lt2 κ2) | 9 := λ T, i2p (weak_subltype_shr_evar_lft E L lt1 lt2 k κ1 κ2 r1 r2 T).
+
+  Lemma mut_subltype_shr E L {rt} (lt1 lt2 : ltype rt) κ1 κ2 T :
+    ⌜lctx_lft_incl E L κ1 κ2⌝ ∗ ⌜lctx_lft_incl E L κ2 κ1⌝ ∗ mut_eqltype E L lt1 lt2 T
+    ⊢ mut_subltype E L (ShrLtype lt1 κ1) (ShrLtype lt2 κ2) T.
+  Proof.
+    iIntros "(%Hsub1 & %Hsub2 & %Heq & $)".
+    iPureIntro. by eapply shr_full_subltype.
+  Qed.
+  Global Instance mut_subltype_shr_inst E L {rt} (lt1 lt2 : ltype rt) κ1 κ2 :
+    MutSubLtype E L (ShrLtype lt1 κ1) (ShrLtype lt2 κ2) | 10 := λ T, i2p (mut_subltype_shr E L lt1 lt2 κ1 κ2 T).
+
+  Lemma mut_subltype_shr_evar_lft E L {rt} (lt1 lt2 : ltype rt) κ1 κ2 T `{!IsProtected κ2} :
+    ⌜κ1 = κ2⌝ ∗ mut_subltype E L (ShrLtype lt1 κ1) (ShrLtype lt2 κ1) T
+    ⊢ mut_subltype E L (ShrLtype lt1 κ1) (ShrLtype lt2 κ2) T.
+  Proof. iIntros "(<- & $)". Qed.
+  Global Instance mut_subltype_shr_evar_lft_inst E L {rt} (lt1 lt2 : ltype rt) κ1 κ2 `{!IsProtected κ2} :
+    MutSubLtype E L (ShrLtype lt1 κ1) (ShrLtype lt2 κ2) | 9 := λ T, i2p (mut_subltype_shr_evar_lft E L lt1 lt2 κ1 κ2 T).
+
+  Lemma mut_eqltype_shr E L {rt} (lt1 lt2 : ltype rt) κ1 κ2 T :
+    ⌜lctx_lft_incl E L κ1 κ2⌝ ∗ ⌜lctx_lft_incl E L κ2 κ1⌝ ∗ mut_eqltype E L lt1 lt2 T
+    ⊢ mut_eqltype E L (ShrLtype lt1 κ1) (ShrLtype lt2 κ2) T.
+  Proof.
+    iIntros "(%Heq1 & %Heq2 & %Heq & $)".
+    iPureIntro. by eapply shr_full_eqltype.
+  Qed.
+  Global Instance mut_eqltype_shr_inst E L {rt} (lt1 lt2 : ltype rt) κ1 κ2 :
+    MutEqLtype E L (ShrLtype lt1 κ1) (ShrLtype lt2 κ2) | 10 := λ T, i2p (mut_eqltype_shr E L lt1 lt2 κ1 κ2 T).
+
+  Lemma mut_eqltype_shr_evar_lft E L {rt} (lt1 lt2 : ltype rt) κ1 κ2 T `{!IsProtected κ2} :
+    ⌜κ1 = κ2⌝ ∗ mut_eqltype E L (ShrLtype lt1 κ1) (ShrLtype lt2 κ1) T
+    ⊢ mut_eqltype E L (ShrLtype lt1 κ1) (ShrLtype lt2 κ2) T.
+  Proof. iIntros "(<- & $)". Qed.
+  Global Instance mut_eqltype_shr_evar_lft_inst E L {rt} (lt1 lt2 : ltype rt) κ1 κ2 `{!IsProtected κ2} :
+    MutEqLtype E L (ShrLtype lt1 κ1) (ShrLtype lt2 κ2) := λ T, i2p (mut_eqltype_shr_evar_lft E L lt1 lt2 κ1 κ2 T).
+
+  (* Ofty unfolding if necessary *)
+  Lemma weak_subltype_shr_ofty_1_evar E L {rt1 rt2} `{!Inhabited rt2} (lt1 : ltype rt1) (ty2 : type (place_rfn rt2)) k κ1 r1 r2 T :
+    (∃ ty2', ⌜ty2 = shr_ref ty2' κ1⌝ ∗ weak_subltype E L k r1 r2 (ShrLtype lt1 κ1) (◁ (shr_ref ty2' κ1)) T)
+    ⊢ weak_subltype E L k r1 r2 (ShrLtype lt1 κ1) (◁ ty2) T.
+  Proof.
+    iIntros "(%ty2' & -> & HT)". done.
+  Qed.
+  Global Instance weak_subltype_shr_ofty_1_evar_inst E L {rt1 rt2} `{!Inhabited rt2} (lt1 : ltype rt1) (ty2 : type (place_rfn rt2)) k κ1 r1 r2 `{!IsProtected ty2} :
+    SubLtype E L k r1 r2 (ShrLtype lt1 κ1) (◁ ty2)%I | 10 := λ T, i2p (weak_subltype_shr_ofty_1_evar E L lt1 ty2 k κ1 r1 r2 T).
+
+  Lemma weak_subltype_shr_ofty_1 E L {rt1 rt2} `{!Inhabited rt2} (lt1 : ltype rt1) (ty2 : type (rt2)) k κ1 κ2 r1 r2 T :
+    weak_subltype E L k r1 r2 (ShrLtype lt1 κ1) (ShrLtype (◁ ty2) κ2) T
+    ⊢ weak_subltype E L k r1 r2 (ShrLtype lt1 κ1) (◁ (shr_ref ty2 κ2)) T.
+  Proof.
+    iIntros "HT". iIntros (??) "#CTX #HE HL".
+    iMod ("HT" with "[//] CTX HE HL") as "(Hincl & $ & $)".
+    iApply (ltype_incl_trans with "Hincl").
+    iApply shr_ref_unfold_1.
+  Qed.
+  Global Instance weak_subltype_shr_ofty_1_inst E L {rt1 rt2} `{!Inhabited rt2} (lt1 : ltype (rt1)) (ty2 : type rt2) k r1 r2 κ1 κ2 :
+    SubLtype E L k r1 r2 (ShrLtype lt1 κ1) (◁ (shr_ref ty2 κ2))%I | 12 := λ T, i2p (weak_subltype_shr_ofty_1 E L lt1 ty2 k κ1 κ2 r1 r2 T).
+
+  Lemma weak_subltype_shr_ofty_2 E L {rt1 rt2} `{!Inhabited rt2} (ty1 : type (rt1)) (lt2 : ltype rt2) k r1 r2 κ1 κ2 T :
+    (weak_subltype E L k r1 r2 (ShrLtype (◁ ty1) κ1) (ShrLtype lt2 κ2) T)
+    ⊢ weak_subltype E L k r1 r2 (◁ (shr_ref ty1 κ1)) (ShrLtype lt2 κ2) T.
+  Proof.
+    iIntros "HT" (??) "#CTX #HE HL".
+    iMod ("HT" with "[//] CTX HE HL") as "(Hincl & $ & $)".
+    iApply (ltype_incl_trans with "[] Hincl").
+    iApply shr_ref_unfold_2.
+  Qed.
+  Global Instance weak_subltype_shr_ofty_2_inst E L {rt1 rt2} `{!Inhabited rt2} (ty1 : type (rt1)) (lt2 : ltype rt2) k r1 r2 κ1 κ2 :
+    SubLtype E L k r1 r2 (◁ (shr_ref ty1 κ1))%I (ShrLtype lt2 κ2) | 10 := λ T, i2p (weak_subltype_shr_ofty_2 E L ty1 lt2 k r1 r2 κ1 κ2 T).
+
+  (* same for [mut_subltype] *)
+  Lemma mut_subltype_shr_ofty_1_evar E L {rt} `{!Inhabited rt} (lt1 : ltype rt) (ty2 : type (place_rfn rt))  κ1 T :
+    (∃ ty2', ⌜ty2 = shr_ref ty2' κ1⌝ ∗ mut_subltype E L (ShrLtype lt1 κ1) (◁ (shr_ref ty2' κ1)) T)
+    ⊢ mut_subltype E L (ShrLtype lt1 κ1) (◁ ty2) T.
+  Proof.
+    iIntros "(%ty2' & -> & HT)". done.
+  Qed.
+  Global Instance mut_subltype_shr_ofty_1_evar_inst E L {rt} `{!Inhabited rt} (lt1 : ltype rt) (ty2 : type (place_rfn rt)) κ1 `{!IsProtected ty2} :
+    MutSubLtype E L (ShrLtype lt1 κ1) (◁ ty2)%I | 10 := λ T, i2p (mut_subltype_shr_ofty_1_evar E L lt1 ty2 κ1 T).
+
+  Lemma mut_subltype_shr_ofty_1 E L {rt} `{!Inhabited rt} (lt1 : ltype rt) (ty2 : type (rt)) κ1 κ2 T :
+    mut_subltype E L (ShrLtype lt1 κ1) (ShrLtype (◁ ty2) κ2) T
+    ⊢ mut_subltype E L (ShrLtype lt1 κ1) (◁ (shr_ref ty2 κ2)) T.
+  Proof.
+    iIntros "(%Hsub & $)". iPureIntro.
+    etrans; first done. eapply full_eqltype_subltype_l. by eapply shr_ref_unfold_full_eqltype.
+  Qed.
+  Global Instance mut_subltype_shr_ofty_1_inst E L {rt} `{!Inhabited rt} (lt1 : ltype (rt)) (ty2 : type rt) κ1 κ2 :
+    MutSubLtype E L (ShrLtype lt1 κ1) (◁ (shr_ref ty2 κ2))%I | 12 := λ T, i2p (mut_subltype_shr_ofty_1 E L lt1 ty2 κ1 κ2 T).
+
+  Lemma mut_subltype_shr_ofty_2 E L {rt} `{!Inhabited rt} (ty1 : type rt) (lt2 : ltype rt) κ1 κ2 T :
+    (mut_subltype E L (ShrLtype (◁ ty1) κ1) (ShrLtype lt2 κ2) T)
+    ⊢ mut_subltype E L (◁ (shr_ref ty1 κ1)) (ShrLtype lt2 κ2) T.
+  Proof.
+    iIntros "(%Hsub & $)". iPureIntro.
+    etrans; last done. eapply full_eqltype_subltype_r. by eapply shr_ref_unfold_full_eqltype.
+  Qed.
+  Global Instance mut_subltype_shr_ofty_2_inst E L {rt} `{!Inhabited rt} (ty1 : type rt) (lt2 : ltype rt) κ1 κ2 :
+    MutSubLtype E L (◁ (shr_ref ty1 κ1))%I (ShrLtype lt2 κ2) | 10 := λ T, i2p (mut_subltype_shr_ofty_2 E L ty1 lt2 κ1 κ2 T).
+
+  (* same for [mut_eqltype] *)
+  Lemma mut_eqltype_shr_ofty_1_evar E L {rt} `{!Inhabited rt} (lt1 : ltype rt) (ty2 : type (place_rfn rt))  κ1 T :
+    (∃ ty2', ⌜ty2 = shr_ref ty2' κ1⌝ ∗ mut_eqltype E L (ShrLtype lt1 κ1) (◁ (shr_ref ty2' κ1)) T)
+    ⊢ mut_eqltype E L (ShrLtype lt1 κ1) (◁ ty2) T.
+  Proof.
+    iIntros "(%ty2' & -> & HT)". done.
+  Qed.
+  Global Instance mut_eqltype_shr_ofty_1_evar_inst E L {rt} `{!Inhabited rt} (lt1 : ltype rt) (ty2 : type (place_rfn rt)) κ1 `{!IsProtected ty2} :
+    MutEqLtype E L (ShrLtype lt1 κ1) (◁ ty2)%I | 10 := λ T, i2p (mut_eqltype_shr_ofty_1_evar E L lt1 ty2 κ1 T).
+
+  Lemma mut_eqltype_shr_ofty_1 E L {rt} `{!Inhabited rt} (lt1 : ltype rt) (ty2 : type (rt)) κ1 κ2 T :
+    mut_eqltype E L (ShrLtype lt1 κ1) (ShrLtype (◁ ty2) κ2) T
+    ⊢ mut_eqltype E L (ShrLtype lt1 κ1) (◁ (shr_ref ty2 κ2)) T.
+  Proof.
+    iIntros "(%Heq & $)". iPureIntro.
+    etrans; first done. by eapply shr_ref_unfold_full_eqltype.
+  Qed.
+  Global Instance mut_eqltype_shr_ofty_1_inst E L {rt} `{!Inhabited rt} (lt1 : ltype (rt)) (ty2 : type rt) κ1 κ2 :
+    MutEqLtype E L (ShrLtype lt1 κ1) (◁ (shr_ref ty2 κ2))%I | 12 := λ T, i2p (mut_eqltype_shr_ofty_1 E L lt1 ty2 κ1 κ2 T).
+
+  Lemma mut_eqltype_shr_ofty_2 E L {rt} `{!Inhabited rt} (ty1 : type rt) (lt2 : ltype rt) κ1 κ2 T :
+    (mut_eqltype E L (ShrLtype (◁ ty1) κ1) (ShrLtype lt2 κ2) T)
+    ⊢ mut_eqltype E L (◁ (shr_ref ty1 κ1)) (ShrLtype lt2 κ2) T.
+  Proof.
+    iIntros "(%Heq & $)". iPureIntro.
+    etrans; last done. symmetry. by eapply shr_ref_unfold_full_eqltype.
+  Qed.
+  Global Instance mut_eqltype_shr_ofty_2_inst E L {rt} `{!Inhabited rt} (ty1 : type rt) (lt2 : ltype rt) κ1 κ2 :
+    MutEqLtype E L (◁ (shr_ref ty1 κ1))%I (ShrLtype lt2 κ2) | 10 := λ T, i2p (mut_eqltype_shr_ofty_2 E L ty1 lt2 κ1 κ2 T).
+
+  (** shortenlft *)
+  (*
+  Lemma type_shortenlft_shr E L sup_lfts {rt} `{!Inhabited rt} (ty : type rt) r κ π v T :
+    (∃ M κs, named_lfts M ∗ ⌜lookup_named_lfts M sup_lfts = Some κs⌝ ∗
+      ⌜lctx_lft_incl E L (lft_intersect_list' κs) κ⌝ ∗
+      (named_lfts M -∗ v ◁ᵥ{π} r @ shr_ref ty (lft_intersect_list' κs) -∗ T L)) -∗
+    typed_annot_expr E L 0 (ShortenLftAnnot sup_lfts) v (v ◁ᵥ{π} r @ shr_ref ty κ) T.
+  Proof.
+    iIntros "(%M & %κs & Hnamed & % & %Hincl & HT)".
+    iIntros "#CTX #HE HL Hv /=".
+    iPoseProof (lctx_lft_incl_incl with "HL HE") as "#Hsyn"; first done.
+    iModIntro. iExists L. iFrame "HL". iApply ("HT" with "Hnamed").
+    unshelve iApply (shr_ref_own_val_mono with "[//] [] Hv"); first done.
+    iIntros (?). iApply type_incl_refl.
+  Qed.
+  Global Instance type_shortenlft_shr_inst E L sup_lfts {rt} `{Inhabited rt} (ty : type rt) r κ π v :
+    TypedAnnotExpr E L 0 (ShortenLftAnnot sup_lfts) v (v ◁ᵥ{π} r @ shr_ref ty κ) :=
+    λ T, i2p (type_shortenlft_shr E L sup_lfts ty r κ π v T).
+   *)
+End rules.
